Parameterize all reasoning rules by thread ids.

coq-osiris/theories/program_logic/fun_spec.v
@@ -93,28 +93,28 @@ Section ewp_spec.
   | type_nel.Tcons X τ', c, P :=
       ∀ (x : X), EWP (call c #x) <|⊥|> {{ ensures c, iSpec τ' c (P x) }}.
 
-  Local Lemma ewp_eval_anon_unary `{Encode X}
+  Local Lemma ewp_eval_anon_unary `{Encode X} ι
     (P : τ[X] -#> microvx -> iProp Σ) η (x : var) e E Ψ
     :
     (∀ (v : X), P v (please_eval ((x, #v) :: η) e)) -∗
-    EWP (eval η (EAnonFun (AnonFun x e))) @ E <| Ψ |> {{ ensures c, iSpec τ[X] c P }}.
+    EWP[ι] (eval η (EAnonFun (AnonFun x e))) @ E <| Ψ |> {{ ensures c, iSpec τ[X] c P }}.
   Proof.
     iIntros "HP"; simpl_eval.
     iApply ewp_ret.
     iApply "HP".
   Qed.
 
-  Local Lemma ewp_eval_anon_binary `{Encode X, Encode Y}
+  Local Lemma ewp_eval_anon_binary `{Encode X, Encode Y} ι
     (P : τ[X;Y] -#> microvx -> iProp Σ) η (x y : var) e E Ψ
     :
     (∀ (vx : X) (vy : Y), P vx vy (please_eval ((y, #vy) :: (x, #vx) :: η) e)) -∗
-    EWP (eval η (EAnonFun (AnonFun x (EAnonFun (AnonFun y e))))) @ E <| Ψ |> {{ ensures c, iSpec τ[X;Y] c P }}.
+    EWP[ι] (eval η (EAnonFun (AnonFun x (EAnonFun (AnonFun y e))))) @ E <| Ψ |> {{ ensures c, iSpec τ[X;Y] c P }}.
   Proof.
     iIntros "HP"; simpl_eval.
     iApply ewp_ret. simpl; simp iSpec.
-    iIntros (vx). simpl.
+    iIntros (vx) "%ι'". simpl.
     iApply ewp_please. iNext.
-    iApply ewp_eval_anon_unary.
+    iApply (ewp_eval_anon_unary ι').
     iIntros (vy).
     iApply "HP".
   Qed.
@@ -130,7 +130,7 @@ Section ewp_spec.
     induction τ as [ | X HX arg_τ IH ]; iIntros (c) "HP Hmono".
     { simp iSpec. iIntros (x).
       iApply "Hmono". iApply "HP". }
-    simp iSpec; iIntros (x).
+    simp iSpec; iIntros (x) "%ι".
     iApply (ewp_mono with "HP").
     iIntros ([c'| ]); [ | iIntros ([])].
     iIntros "HSpec'". simpl.
@@ -184,7 +184,7 @@ Section ewp_spec.
     iIntros "HP".
     destruct τ as [ X | X HX τ ].
     { iApply "HP". }
-    simp iSpec; iIntros (vx).
+    simp iSpec; iIntros (vx) "%ι".
     simp predicate_over_function_body.
     iSpecialize ("HP" $! vx).
     iPoseProof (invert_predicate_over_body with "HP") as "(%y & %e' & ->)".
@@ -199,11 +199,12 @@ Section ewp_spec.
   Lemma ewp_eval_anon
     (τ : types)
     (P : τ -#> microvx -> iProp Σ)
+    ι
     η
     (x : var)
     e E Ψ :
     predicate_over_function_body τ P η (EAnonFun (AnonFun x e)) -∗
-    EWP (eval η (EAnonFun (AnonFun x e))) @ E <| Ψ |> {{ ensures c, iSpec τ c P }}.
+    EWP[ι] (eval η (EAnonFun (AnonFun x e))) @ E <| Ψ |> {{ ensures c, iSpec τ c P }}.
   Proof.
     iIntros "HP".
     simpl_eval; iApply ewp_ret; simpl.
@@ -248,7 +249,7 @@ Section ewp_spec.
       iIntros (x).
       iPureIntro.
       apply HSpec. }
-    simp iSpec. iIntros (x). simp Spec in HSpec.
+    simp iSpec. iIntros (x) "%ι". simp Spec in HSpec.
     specialize (HSpec x).
     destruct c; simpl in HSpec; try by apply invert_pure_wp_crash in HSpec.
     - destruct a; simpl in *.
@@ -277,11 +278,11 @@ Section ewp_spec.
 
   (* [ewp_EApp_partial] is a lemma for partial application. *)
 
-  Lemma ewp_EApp_partial `{Encode X} (τ: types) η e e1 Ψ
+  Lemma ewp_EApp_partial `{Encode X} (τ: types) ι η e e1 Ψ
     (P : type_nel.Tcons X τ -#> microvx -> iProp Σ) :
-    EWP eval η e <|Ψ|> {{ ensures c, iSpec (type_nel.Tcons X τ) c P }} -∗
-    EWP eval η e1 <|Ψ|> {{ ensures v1, ∃ (x : X), ⌜v1 = #x⌝ }} -∗
-    EWP eval η (EApp e e1) <|Ψ|> {{ ensures c, ∃ (x : X), iSpec τ c (P x) }}.
+    EWP[ι] eval η e <|Ψ|> {{ ensures c, iSpec (type_nel.Tcons X τ) c P }} -∗
+    EWP[ι] eval η e1 <|Ψ|> {{ ensures v1, ∃ (x : X), ⌜v1 = #x⌝ }} -∗
+    EWP[ι] eval η (EApp e e1) <|Ψ|> {{ ensures c, ∃ (x : X), iSpec τ c (P x) }}.
   Proof.
     iIntros "He He1". simpl_eval.
     iApply (ewp_Par with "He He1").
@@ -307,7 +308,7 @@ End ewp_spec.
 Section ewp_EApp_prop_aux_def.
 
   Context `{!osirisGS Σ}.
-  Context (η : env) (Ψ : iEff Σ).
+  Context (ι : thread) (η : env) (Ψ : iEff Σ).
   Context (expr_base : expr) (goal_prop : expr -> iProp Σ).
 
   (* [accumulate_argument_premises_and_build_consequence_hyp] builds up
@@ -318,7 +319,7 @@ Section ewp_EApp_prop_aux_def.
     iProp Σ :=
   | Tbase X, es, conseq_acc :=
       ∀ (e : expr) (φ : X -> iProp Σ),
-        EWP eval η e <|Ψ|> {{ ensures #x, φ x }} -∗
+        EWP[ι] eval η e <|Ψ|> {{ ensures #x, φ x }} -∗
         (* [Hconseq] is the consequence premise built over all parameters *)
         let Hconseq := ∀ (x : X), conseq_acc x (φ x) in
         (* [nested_eapp] is the nested application *)
@@ -326,7 +327,7 @@ Section ewp_EApp_prop_aux_def.
         Hconseq -∗ goal_prop (nested_eapp)
   | type_nel.Tcons X τ', es, conseq_acc :=
       ∀ (e : expr) (φ : X -> iProp Σ),
-        EWP eval η e <|Ψ|> {{ ensures #x, φ x }} -∗
+        EWP[ι] eval η e <|Ψ|> {{ ensures #x, φ x }} -∗
         let conseq_acc :=
           (λ# (tt : τ') (Q : iProp Σ),
               ∀ (x : X),
@@ -368,16 +369,16 @@ Section ewp_EApp_def.
   Context `{!osirisGS Σ}.
 
   Definition ewp_EApp_prop `{Encode A} (τ : types) : iProp Σ :=
-    ∀ (η : env) (e : expr) (Ψ' : A -> iProp Σ) (Ψ : iEff Σ)
+    ∀ (ι : thread) (η : env) (e : expr) (Ψ' : A -> iProp Σ) (Ψ : iEff Σ)
       (P : τ -#> microvx -> iProp Σ),
-    EWP eval η e <|Ψ|> {{ ensures c, iSpec τ c P }} -∗
+    EWP[ι] eval η e <|Ψ|> {{ ensures c, iSpec τ c P }} -∗
     accumulate_argument_premises_and_build_consequence_hyp
-      η Ψ e
-      (λ e, EWP eval η e <|Ψ|> {{ ensures #v, Ψ' v }})
+      ι η Ψ e
+      (λ e, EWP[ι] eval η e <|Ψ|> {{ ensures #v, Ψ' v }})
       τ
       []
       (λ# (tt : τ) (Q : iProp Σ),
-           Q -∗ ∀ m, (tapp P tt) m -∗ ▷ EWP m <|Ψ|> {{ ensures #v, Ψ' v }}).
+           Q -∗ ∀ m, (tapp P tt) m -∗ ▷ EWP[ι] m <|Ψ|> {{ ensures #v, Ψ' v }}).
 
   Arguments ewp_EApp_prop {_ _} !τ /.
   Transparent ewp_EApp_prop.
@@ -386,13 +387,13 @@ Section ewp_EApp_def.
   (* Helper lemma for the induction step *)
 
   Lemma ewp_EApp_prop_induction_step
-    (τ : types) (η : env) (Ψ : iEff Σ) e (g : expr -> iProp Σ) :
+    (τ : types) ι (η : env) (Ψ : iEff Σ) e (g : expr -> iProp Σ) :
     ∀ (Hconseq : τ -#> iProp Σ -> iProp Σ) (es : list expr) (ei : expr),
       app_exprs (EApp e ei) es = app_exprs e (es ++ [ei]) →
       accumulate_argument_premises_and_build_consequence_hyp
-        η Ψ (EApp e ei) g τ es Hconseq -∗
+        ι η Ψ (EApp e ei) g τ es Hconseq -∗
       accumulate_argument_premises_and_build_consequence_hyp
-        η Ψ e g τ (es ++ [ei]) Hconseq.
+        ι η Ψ e g τ (es ++ [ei]) Hconseq.
   Proof.
     induction τ as [ X HX | X HX τ IH ]; iIntros (Hconseq es ei HeqEApp) "Happlied".
     - (* Base case *)
@@ -408,8 +409,6 @@ Section ewp_EApp_def.
       + iApply ("Happlied" with "Hex").
   Qed.
 
-
-
   (* Main lemma for n-ary function application *)
 
   Lemma ewp_EApp `{Encode A} (τ : types) :
@@ -418,7 +417,7 @@ Section ewp_EApp_def.
     induction τ as [ X HX | X HX τ IH].
     - (* Base case *)
       unfold ewp_EApp_prop.
-      iIntros (η e Ψ' Ψ P) "HSpec"; iIntros (ex φx) "Hex"; cbn zeta.
+      iIntros (ι η e Ψ' Ψ P) "HSpec"; iIntros (ex φx) "Hex"; cbn zeta.
       iIntros "Hmono".
       simpl_eval.
       iApply (ewp_Par with "HSpec Hex").
@@ -430,10 +429,10 @@ Section ewp_EApp_def.
 
     - (* Inductive case: multi-argument function *)
       unfold ewp_EApp_prop.
-      iIntros (η e Ψ' Ψ P) "HSpec"; iIntros (ex φx) "Hex".
+      iIntros (ι η e Ψ' Ψ P) "HSpec"; iIntros (ex φx) "Hex".
       change [ex] with ([] ++ [ex]).
-    iApply (ewp_EApp_prop_induction_step τ η Ψ e
-              (λ e, EWP eval η e <|Ψ|> {{ ensures #x, Ψ' x }})%I); first reflexivity.
+      iApply (ewp_EApp_prop_induction_step τ ι η Ψ e
+              (λ e, EWP[ι] eval η e <|Ψ|> {{ ensures #x, Ψ' x }})%I); first reflexivity.
 
     (* Define the intermediate specification P' *)
     set (P' := (λ# (tt : τ) m,
@@ -444,15 +443,13 @@ Section ewp_EApp_def.
     (* Use IH *)
     iPoseProof IH as "HIH".
     unfold ewp_EApp_prop.
-    iSpecialize ("HIH" $! η (EApp e ex) _ _ P' with "[HSpec Hex]").
+    iSpecialize ("HIH" $! ι η (EApp e ex) _ _ P' with "[HSpec Hex]").
     { simpl_eval.
       iApply (prove_ewp_Par with "HSpec Hex").
       iIntros (??) "HSpec (%x & -> & Hφx) /=".
       simp iSpec.
-      iIntros (ι).
-      iSpecialize ("HSpec" $! x ι).
-      iPoseProof (ewpi_prot_mono with "[] HSpec") as "HSpec"; last first.
-      iApply (ewpi_mono with "HSpec").
+      iPoseProof (ewp_prot_mono with "[] HSpec") as "HSpec"; last first.
+      iApply (ewp_mono with "HSpec").
       iIntros ([|]); [ | iIntros ([]) ].
       iIntros "HSpec /=".
       iApply (iSpec_mono with "HSpec").
@@ -473,7 +470,7 @@ Section ewp_EApp_def.
 
 End ewp_EApp_def.
 
-Section ewpi_EApp_prop_aux_def.
+Section ewp_EApp_prop_aux_def.
 
   Context `{!osirisGS Σ}.
   Context (ι : thread) (η : env) (Ψ : iEff Σ).
@@ -509,135 +506,4 @@ Section ewpi_EApp_prop_aux_def.
   Transparent iaccumulate_argument_premises_and_build_consequence_hyp.
   Strategy transparent [ iaccumulate_argument_premises_and_build_consequence_hyp ].
 
-  (* Monotonicity of the accumulator *)
-
-  Lemma ewpi_EApp_mono (τ : types) es (Hmon' Hmon : τ -#> iProp Σ -> iProp Σ) :
-    iaccumulate_argument_premises_and_build_consequence_hyp τ es Hmon' -∗
-    □ (∀ args (P : iProp Σ), Hmon args P -∗ Hmon' args P) -∗
-    iaccumulate_argument_premises_and_build_consequence_hyp τ es Hmon.
-  Proof.
-    revert es.
-    induction τ as [ X HX | X HX τ IH ]; iIntros (es) "HEApp' #Hmono"; simpl.
-    - iIntros (ex φx) "Hex Hx". cbn zeta.
-      iSpecialize ("HEApp'" $! ex φx with "Hex"). cbn zeta.
-      iApply "HEApp'".
-      iIntros (v). iApply ("Hmono" with "Hx").
-    - iIntros (ex φx) "Hex".
-      iApply (IH with "[HEApp' Hex]").
-      + iApply ("HEApp'" with "Hex").
-      + iModIntro. iIntros (args P). rewrite !tapp_bind.
-        iIntros "Hx" (x) "Hφx".
-        iApply ("Hmono" $! (x, args) P).
-        iApply ("Hx" with "Hφx").
-  Qed.
-
-End ewpi_EApp_prop_aux_def.
-
-Section ewpi_EApp_def.
-  Context `{!osirisGS Σ}.
-
-  Definition ewpi_EApp_prop `{Encode A} (τ : types) : iProp Σ :=
-    ∀ (ι : thread) (η : env) (e : expr) (Ψ' : A -> iProp Σ) (Ψ : iEff Σ)
-      (P : τ -#> microvx -> iProp Σ),
-    EWP[ι] eval η e <|Ψ|> {{ ensures c, iSpec τ c P }} -∗
-    iaccumulate_argument_premises_and_build_consequence_hyp
-      ι η Ψ e
-      (λ e, EWP[ι] eval η e <|Ψ|> {{ ensures #v, Ψ' v }})
-      τ
-      []
-      (λ# (tt : τ) (Q : iProp Σ),
-           Q -∗ ∀ m, (tapp P tt) m -∗ ▷ EWP[ι] m <|Ψ|> {{ ensures #v, Ψ' v }}).
-
-  Arguments ewpi_EApp_prop {_ _} !τ /.
-  Transparent ewpi_EApp_prop.
-  Strategy transparent [ ewpi_EApp_prop ].
-
-  (* Helper lemma for the induction step *)
-
-  Lemma ewpi_EApp_prop_induction_step
-    ι (τ : types) (η : env) (Ψ : iEff Σ) e (g : expr -> iProp Σ) :
-    ∀ (Hconseq : τ -#> iProp Σ -> iProp Σ) (es : list expr) (ei : expr),
-      app_exprs (EApp e ei) es = app_exprs e (es ++ [ei]) →
-      iaccumulate_argument_premises_and_build_consequence_hyp
-        ι η Ψ (EApp e ei) g τ es Hconseq -∗
-      iaccumulate_argument_premises_and_build_consequence_hyp
-        ι η Ψ e g τ (es ++ [ei]) Hconseq.
-  Proof.
-    induction τ as [ X HX | X HX τ IH ]; iIntros (Hconseq es ei HeqEApp) "Happlied".
-    - (* Base case *)
-      simpl in *. rewrite <- HeqEApp. iApply "Happlied".
-    - (* Inductive case *)
-      iIntros (ex φx) "Hex". cbn zeta.
-      iApply (IH (λ# (tt : τ) (B : iProp Σ),
-                   ∀ x : X,
-                     φx x -∗
-                     tapp Hconseq (x, tt) B)%I
-                 (ex :: es) ei).
-      + simpl. f_equal. apply HeqEApp.
-      + iApply ("Happlied" with "Hex").
-  Qed.
-
-  (* Main lemma for n-ary function application *)
-
-  Lemma ewpi_EApp `{Encode A} (τ : types) :
-    ⊢ @ewpi_EApp_prop A _ τ.
-  Proof.
-    induction τ as [ X HX | X HX τ IH].
-    - (* Base case *)
-      unfold ewp_EApp_prop.
-      iIntros (ι η e Ψ' Ψ P) "HSpec"; iIntros (ex φx) "Hex"; cbn zeta.
-      iIntros "Hmono".
-      simpl_eval.
-      iApply (ewpi_Par with "HSpec Hex").
-      + iIntros (?) "[]".
-      + iIntros (?) "[]".
-      + iIntros (c v) "HSpec' Hφx". simpl. simp iSpec.
-        iDestruct "Hφx" as (x) "[-> Hφx]".
-        iApply ("Hmono" with "Hφx HSpec'").
-
-    - (* Inductive case: multi-argument function *)
-      unfold ewpi_EApp_prop.
-      iIntros (ι η e Ψ' Ψ P) "HSpec"; iIntros (ex φx) "Hex".
-      change [ex] with ([] ++ [ex]).
-    iApply (ewpi_EApp_prop_induction_step ι τ η Ψ e
-              (λ e, EWP[ι] eval η e <|Ψ|> {{ ensures #x, Ψ' x }})%I); first reflexivity.
-
-    (* Define the intermediate specification P' *)
-    set (P' := (λ# (tt : τ) m,
-                 ∃ x : X,
-                   φx x ∗
-                   tapp P (x, tt) m)%I : τ -#> microvx -> iProp Σ).
-
-    (* Use IH *)
-    iPoseProof IH as "HIH".
-    unfold ewp_EApp_prop.
-    iSpecialize ("HIH" $! ι η (EApp e ex) _ _ P' with "[HSpec Hex]").
-    { simpl_eval.
-      iApply (ewpi_Par with "HSpec Hex").
-      - iIntros (? []).
-      - iIntros (? []).
-      -
-        iIntros (??) "HSpec (%x & -> & Hφx) /=".
-        simp iSpec.
-        iSpecialize ("HSpec" $! x ι).
-        iPoseProof (ewpi_prot_mono with "[] HSpec") as "HSpec"; last first.
-        iApply (ewpi_mono with "HSpec").
-        iIntros ([|]); [ | iIntros ([]) ].
-        iIntros "!> HSpec /=".
-        iApply (iSpec_mono with "HSpec").
-        rewrite bi_tforall_equiv.
-        iIntros (xs m) "HP".
-        subst P'. cbn. rewrite tapp_bind.
-        iFrame. iApply iEff_le_bottom. }
-
-    (* Apply monotonicity *)
-    iApply (ewpi_EApp_mono with "HIH").
-
-    iIntros "!>" (args Q). rewrite !tapp_bind.
-    iIntros "H HQ %m (%x & Hφx & HP)".
-    iSpecialize ("H" $! x with "Hφx").
-    rewrite tapp_bind.
-    iApply ("H" with "HQ HP").
-  Qed.
-
-End ewpi_EApp_def.
+End ewp_EApp_prop_aux_def.
