coq-osiris/theories/program_logic/expr_rules.v
@@ -19,6 +19,8 @@ Section ewp_binding_rules.
 
   Context `{!osirisGS Σ}.
 
+  Context {ι : thread}.
+
   (* -------------------------------------------------------------------------- *)
   (* Auxiliary lemmas that are useful when proving facts about [EWP eval _] *)
 
@@ -26,7 +28,7 @@ Section ewp_binding_rules.
   Lemma ewp_widen {A E} (e : micro A void.void) Ψ m φ φ' :
     pure_wp e φ ⊥ ->
     (∀ v, ⌜φ v⌝ -∗ φ' (O2Ret v)) -∗
-    EWP (widen e : micro A E) @ m <|Ψ|> {{ φ' }}.
+    EWP[ι] (widen e : micro A E) @ m <|Ψ|> {{ φ' }}.
   Proof.
     iIntros (He) "H".
     iApply ewp_mono.
@@ -39,11 +41,11 @@ Section ewp_binding_rules.
 
   Lemma ewp_eval_bindings_cons_total η p e bs
     (φ1 : val -> iProp Σ) (φs : val -> env -> Prop) (φ φ' : env -> iProp Σ) E Ψ :
-    EWP eval η e @ E <|Ψ|> {{ ensures v, φ1 v }} -∗
-    EWP eval_bindings η bs @ E <|Ψ|> {{ ensures v, φ v }} -∗
+    EWP[ι] eval η e @ E <|Ψ|> {{ ensures v, φ1 v }} -∗
+    EWP[ι] eval_bindings η bs @ E <|Ψ|> {{ ensures v, φ v }} -∗
     (∀ v δ, φ1 v -∗ φ δ -∗ ⌜pure_wp (irrefutably_extend η δ p v) (φs v) ⊥⌝) -∗
     (∀ v δ, φ1 v -∗  ⌜φs v δ⌝ -∗ φ' δ) -∗
-    EWP eval_bindings η (Binding p e :: bs) @ E <|Ψ|> {{ ensures v, φ' v }}.
+    EWP[ι] eval_bindings η (Binding p e :: bs) @ E <|Ψ|> {{ ensures v, φ' v }}.
   Proof.
     iIntros "H1 H2 P Hcons /=".
     simpl_eval_bindings.
@@ -58,16 +60,16 @@ Section ewp_binding_rules.
   Qed.
 
   Lemma ewp_eval_bindings_nil η E Ψ :
-    ⊢ EWP eval_bindings η [] @ E <|Ψ|> {{ RET= [] }}.
+    ⊢ EWP[ι] eval_bindings η [] @ E <|Ψ|> {{ RET= [] }}.
   Proof.
     simpl_eval_bindings; by iApply ewp_ret.
   Qed.
 
   Corollary ewp_eval_bindings_singleton_total {η p e} Φ φ φs E Ψ :
-    EWP eval η e @ E <|Ψ|> {{ ensures v, Φ v }} -∗
+    EWP[ι] eval η e @ E <|Ψ|> {{ ensures v, Φ v }} -∗
     (∀ v, Φ v -∗ ⌜pure_wp (irrefutably_extend η nil p v) (φs v) ⊥⌝) -∗
     (∀ v δ, Φ v -∗ ⌜φs v δ⌝ -∗ φ δ) -∗
-    EWP eval_bindings η [ Binding p e ] @ E <|Ψ|> {{ ensures v, φ v }}.
+    EWP[ι] eval_bindings η [ Binding p e ] @ E <|Ψ|> {{ ensures v, φ v }}.
   Proof.
     iIntros "H1 P /=".
     iApply (ewp_eval_bindings_cons_total with "H1").
@@ -77,13 +79,13 @@ Section ewp_binding_rules.
   Qed.
 
   Lemma ewp_eval_bindings_cons η p e bs φ1 φs φ E Ψ :
-    EWP eval η e @ E <|Ψ|> {{ φ1 }} -∗
-    EWP eval_bindings η bs @ E <|Ψ|> {{ φs }} -∗
+    EWP[ι] eval η e @ E <|Ψ|> {{ φ1 }} -∗
+    EWP[ι] eval_bindings η bs @ E <|Ψ|> {{ φs }} -∗
     (∀ v : exn, φ1 (O2Throw v) -∗ φ (O2Throw v)) -∗
     (∀ v : exn, φs (O2Throw v) -∗ φ (O2Throw v)) -∗
     (∀ v δ, φ1 (O2Ret v) ∗ φs (O2Ret δ) -∗
-      EWP widen (irrefutably_extend η δ p v)  @ E <|Ψ|> {{ φ }}) -∗
-    EWP eval_bindings η (Binding p e :: bs) @ E <|Ψ|> {{ φ }}.
+      EWP[ι] widen (irrefutably_extend η δ p v)  @ E <|Ψ|> {{ φ }}) -∗
+    EWP[ι] eval_bindings η (Binding p e :: bs) @ E <|Ψ|> {{ φ }}.
   Proof.
     iIntros "H1 H2 E1 E2 P /=". simpl_eval_bindings.
     iApply (ewp_Par with "H1 H2 [E1] [E2]").
@@ -96,7 +98,7 @@ End ewp_binding_rules.
 
 Section ewp_rules_expr.
 
-  Context `{!osirisGS Σ}.
+  Context `{!osirisGS Σ} {ι : thread}.
 
   (* -------------------------------------------------------------------------- *)
   (* Lemmas about [expr]s *)
@@ -104,8 +106,8 @@ Section ewp_rules_expr.
   (** * EPath : path → expr *)
 
   Lemma ewp_EPath η p φ E Ψ :
-    EWP lookup_path η p @ E <|Ψ|> {{ ensures v, φ v }} -∗
-    EWP eval η (EPath p) @ E <|Ψ|> {{ ensures v, φ v }}.
+    EWP[ι] lookup_path η p @ E <|Ψ|> {{ ensures v, φ v }} -∗
+    EWP[ι] eval η (EPath p) @ E <|Ψ|> {{ ensures v, φ v }}.
   Proof.
     iIntros "H /=". simpl_eval.
     iApply ewp_try.
@@ -114,52 +116,17 @@ Section ewp_rules_expr.
     by iApply ewp_ret.
   Qed.
 
-  Lemma ewpi_EPath ι η p φ E Ψ :
-    EWP[ι] lookup_path η p @ E <|Ψ|> {{ ensures v, φ v }} -∗
-    EWP[ι] eval η (EPath p) @ E <|Ψ|> {{ ensures v, φ v }}.
-  Proof.
-    iIntros "H /=". simpl_eval.
-    iApply ewpi_try.
-    iApply (ewpi_mono with "H").
-    iIntros ([|[]]) "A/=".
-    by iApply ewpi_ret.
-  Qed.
-
-
   (** * EAnonFun : anonfun → expr *)
-
-  Lemma ewp_EAnonFun `{Encode A} η x e φ E Ψ P :
-    ▷ (∀ (vx : A), P vx -∗ EWP eval ((x, #vx)::η) e @ E <| Ψ |> {{ ensures v, φ v }}) -∗
-    EWP eval η (EAnonFun (AnonFun x e)) @ E <| Ψ |> {{ ensures v, ∀ (vx : A), P vx -∗ EWP (call v #vx) @ E <| Ψ |> {{ ensures v, φ v}} }}.
-  Proof.
-    iIntros "H". simpl_eval.
-    iApply ewp_ret. simpl.
-    iIntros (vx) "HP".
-    iApply ewp_please. iModIntro.
-    by iApply "H".
-  Qed.
-
-  Lemma ewp_EAnonFun_partial `{Encode A, Encode B} η x e (φ : B -> iProp Σ) E Ψ P :
-    ▷ (∀ (vx : A), P vx -∗ EWP eval ((x, #vx)::η) e @ E <| Ψ |> {{ ensures #v, φ v }}) -∗
-    EWP eval η (EAnonFun (AnonFun x e)) @ E <| Ψ |> {{ ensures v, ∀ (vx : A), P vx -∗ EWP (call v #vx) @ E <| Ψ |> {{ ensures #v, φ v}} }}.
-  Proof.
-    iIntros "H". simpl_eval.
-    iApply ewp_ret. simpl.
-    iIntros (vx) "HP".
-    iApply ewp_please. iModIntro.
-    by iApply "H".
-  Qed.
-
-
   (** * EApp : expr → expr → expr *)
+  (* See [funspec.v] *)
 
   Lemma ewp_EApp_exn η e1 e2 φ1 φ2 φ E Ψ :
-    EWP eval η e1 @ E <|Ψ|> {{ φ1 }} -∗
-    EWP eval η e2 @ E <|Ψ|> {{ φ2 }} -∗
+    EWP[ι] eval η e1 @ E <|Ψ|> {{ φ1 }} -∗
+    EWP[ι] eval η e2 @ E <|Ψ|> {{ φ2 }} -∗
     (∀ v, φ1 (O2Throw v) -∗ φ (O2Throw v)) -∗
     (∀ v, φ2 (O2Throw v) -∗ φ (O2Throw v)) -∗
-    (∀ v1 v2, φ1 (O2Ret v1) -∗ φ2 (O2Ret v2) -∗ EWP call v1 v2 @ E <|Ψ|> {{ φ }}) -∗
-    EWP eval η (EApp e1 e2) @ E <|Ψ|> {{ φ }}.
+    (∀ v1 v2, φ1 (O2Ret v1) -∗ φ2 (O2Ret v2) -∗ EWP[ι] call v1 v2 @ E <|Ψ|> {{ φ }}) -∗
+    EWP[ι] eval η (EApp e1 e2) @ E <|Ψ|> {{ φ }}.
   Proof.
     iIntros "H1 H2 E1 E2 P /=". simpl_eval.
     iApply (ewp_Par with "H1 H2 [E1] [E2]").
@@ -169,11 +136,11 @@ Section ewp_rules_expr.
   Qed.
 
   Lemma ewp_EApp' η e1 e2 φ1 φ2 φ E Ψ :
-    EWP eval η e1 @ E <|Ψ|> {{ ensures v, φ1 v }} -∗
-    EWP eval η e2 @ E <|Ψ|> {{ ensures v, φ2 v }} -∗
+    EWP[ι] eval η e1 @ E <|Ψ|> {{ ensures v, φ1 v }} -∗
+    EWP[ι] eval η e2 @ E <|Ψ|> {{ ensures v, φ2 v }} -∗
     (∀ v1 v2, φ1 v1 -∗ φ2 v2 -∗
-       EWP call v1 v2 @ E <|Ψ|> {{ φ }}) -∗
-    EWP eval η (EApp e1 e2) @ E <|Ψ|> {{ φ }}.
+       EWP[ι] call v1 v2 @ E <|Ψ|> {{ φ }}) -∗
+    EWP[ι] eval η (EApp e1 e2) @ E <|Ψ|> {{ φ }}.
   Proof.
     iIntros "H1 H2 H".
     iApply (ewp_EApp_exn with "H1 H2"); try iIntros (?) "[]".
@@ -189,30 +156,30 @@ Section ewp_rules_expr.
   might be too verbose or be too trivial, and one could simply wish to "just
   reduce" the term, in which case those lemmas may be useful. *)
   Lemma ewp_call_nonrec η x_arg body v_arg φ E Ψ:
-    ▷EWP eval ((x_arg, v_arg) :: η) body @ E <|Ψ|> {{ φ }} -∗
-    EWP call (VClo η (AnonFun x_arg body)) v_arg @ E <|Ψ|> {{ φ }}.
+    ▷EWP[ι] eval ((x_arg, v_arg) :: η) body @ E <|Ψ|> {{ φ }} -∗
+    EWP[ι] call (VClo η (AnonFun x_arg body)) v_arg @ E <|Ψ|> {{ φ }}.
   Proof.
     iIntros "H".
-    iApply ewp_eval. iNext.
+    iApply ewp_please. iNext.
     iApply (ewp_mono with "H").
-    iIntros ([]). iApply ewp_ret. iApply ewp_throw.
+    iIntros (o) "$".
   Qed.
 
   Lemma ewp_call_rec η f x body bs v φ E Ψ:
     lookup_rec_bindings bs f = ret (AnonFun x body) ->
-    ▷EWP eval ((x, v) :: eval_rec_bindings η bs ++ η) body @ E <|Ψ|> {{ φ }} -∗
-    EWP call (VCloRec η bs f) v @ E <|Ψ|> {{ φ }}.
+    ▷ EWP[ι] eval ((x, v) :: eval_rec_bindings η bs ++ η) body @ E <|Ψ|> {{ φ }} -∗
+    EWP[ι] call (VCloRec η bs f) v @ E <|Ψ|> {{ φ }}.
   Proof.
     iIntros (Hlk) "H /=". rewrite Hlk /=.
-    iApply ewp_eval. iNext.
+    iApply ewp_please. iNext.
     iApply (ewp_mono with "H").
-    iIntros ([]). iApply ewp_ret. iApply ewp_throw.
+    iIntros (o) "$".
   Qed.
 
   Lemma ewp_call_rec_1 η f x body v φ E Ψ:
     let vf := VCloRec η [RecBinding f (AnonFun x body)] f in
-    ▷EWP eval ((x, v) :: (f, vf) :: η) body @ E <|Ψ|> {{ φ }} -∗
-    EWP call vf v @ E <|Ψ|> {{ φ }}.
+    ▷EWP[ι] eval ((x, v) :: (f, vf) :: η) body @ E <|Ψ|> {{ φ }} -∗
+    EWP[ι] call vf v @ E <|Ψ|> {{ φ }}.
   Proof.
     iIntros (vf) "H". iApply ewp_call_rec; auto.
     rewrite /= String.eqb_refl //.
@@ -222,8 +189,8 @@ Section ewp_rules_expr.
 
   Lemma ewp_evals η E es φs φe ψ:
     ([∗ list] ei;φi ∈ es;φs,
-       EWP eval η ei @ E <| ψ |> {{ RET v => φi v | EXN e => φe e }}) -∗
-    EWP evals η es @ E <| ψ |>
+       EWP[ι] eval η ei @ E <| ψ |> {{ RET v => φi v | EXN e => φe e }}) -∗
+    EWP[ι] evals η es @ E <| ψ |>
       {{   RET vs => [∗ list] vi; φi ∈ vs; φs, φi vi
          | EXN e => φe e}}.
   Proof.
@@ -240,14 +207,14 @@ Section ewp_rules_expr.
   Qed.
 
   Lemma ewp_ETuple_forward_exn η es φs φe E Ψ :
-    ([∗ list] ei; φi ∈ es; φs, EWP eval η ei @ E <|Ψ|> {{ RET v => φi v | EXN e => φe e }}) -∗
-    EWP eval η (ETuple es) @ E <|Ψ|>
+    ([∗ list] ei; φi ∈ es; φs, EWP[ι] eval η ei @ E <|Ψ|> {{ RET v => φi v | EXN e => φe e }}) -∗
+    EWP[ι] eval η (ETuple es) @ E <|Ψ|>
       {{  RET v => ∃ vs, ⌜v = VTuple vs⌝ ∗ [∗ list] vi; φi ∈ vs; φs, φi vi
         | EXN e => φe e }}.
   Proof.
     iIntros "H /=". simpl_eval.
-    iApply ewp_bind_exn.
-    iApply (ewp_mono _ _ (  RET vs => [∗ list] vi; φi ∈ vs; φs, φi vi
+    iApply ewp_bind'.
+    iApply (ewp_mono _ _ _ (  RET vs => [∗ list] vi; φi ∈ vs; φs, φi vi
                           | EXN v => φe v) with "[-]")%I.
     2: by iIntros ([]) "A/="; auto; iApply ewp_ret; simpl; iExists _; auto.
     iInduction es as [ | ei es ] "IH" forall (φs) "H"; simpl_evals.
@@ -261,22 +228,22 @@ Section ewp_rules_expr.
   Qed.
 
   Lemma ewp_ETuple_forward η es φs E Ψ :
-    ([∗ list] ei; φi ∈ es; φs, EWP eval η ei @ E <|Ψ|> {{ ensures v, φi v }}) -∗
-    EWP eval η (ETuple es) @ E <|Ψ|>
+    ([∗ list] ei; φi ∈ es; φs, EWP[ι] eval η ei @ E <|Ψ|> {{ ensures v, φi v }}) -∗
+    EWP[ι] eval η (ETuple es) @ E <|Ψ|>
       {{ ensures v, ∃ vs, ⌜v = VTuple vs⌝ ∗ [∗ list] vi; φi ∈ vs; φs, φi vi }}.
   Proof.
     iApply ewp_ETuple_forward_exn.
   Qed.
 
   Lemma ewp_ETuple_exn η es φs φ E Ψ :
-    ([∗ list] ei; φi ∈ es; φs, EWP eval η ei @ E <|Ψ|> {{ φi }}) -∗
+    ([∗ list] ei; φi ∈ es; φs, EWP[ι] eval η ei @ E <|Ψ|> {{ φi }}) -∗
     (∀ vs, ([∗ list] vi; φi ∈ vs; φs, φi (O2Ret vi)) -∗
        φ (O2Ret (VTuple vs))) -∗
     ([∗ list] φi ∈ φs, ∀ e, φi (O2Throw e) -∗ φ (O2Throw e)) -∗
-    EWP eval η (ETuple es) @ E <|Ψ|> {{ φ }}.
+    EWP[ι] eval η (ETuple es) @ E <|Ψ|> {{ φ }}.
   Proof.
     iIntros "H P E". simpl_eval.
-    iApply ewp_bind_exn.
+    iApply ewp_bind'.
     iApply (ewp_mono with "[H E]"); first iApply ewp_evals.
     - iPoseProof (big_sepL2_length with "[$]") as "%".
       setoid_rewrite big_sepL2_fmap_r.
@@ -297,24 +264,24 @@ Section ewp_rules_expr.
 
   (* Results to handle goals generated by ewp_ETuple_* lemmas *)
   Lemma ewp_list_nil η E Ψ :
-    ⊢ ([∗ list] ei;φi ∈ []; [], EWP eval η ei @ E <|Ψ|> {{ φi }}).
+    ⊢ ([∗ list] ei;φi ∈ []; [], EWP[ι] eval η ei @ E <|Ψ|> {{ φi }}).
   Proof. done. Qed.
 
   Lemma ewp_list_cons η e es φ φs E Ψ :
-    EWP eval η e @ E <|Ψ|> {{ φ }} -∗
-    ([∗ list] ei;φi ∈ es;φs, EWP eval η ei @ E <|Ψ|> {{ φi }}) -∗
-    ([∗ list] ei;φi ∈ (e :: es);(φ :: φs), EWP eval η ei @ E <|Ψ|> {{ φi }}).
+    EWP[ι] eval η e @ E <|Ψ|> {{ φ }} -∗
+    ([∗ list] ei;φi ∈ es;φs, EWP[ι] eval η ei @ E <|Ψ|> {{ φi }}) -∗
+    ([∗ list] ei;φi ∈ (e :: es);(φ :: φs), EWP[ι] eval η ei @ E <|Ψ|> {{ φi }}).
   Proof. iIntros "He Hlist". simpl. iFrame. Qed.
 
   Lemma ewp_list_singleton η e φ E Ψ :
-    EWP eval η e @ E <|Ψ|> {{ φ }} -∗
-    ([∗ list] ei;φi ∈ [e]; [φ], EWP eval η ei @ E <|Ψ|> {{ φi }}).
+    EWP[ι] eval η e @ E <|Ψ|> {{ φ }} -∗
+    ([∗ list] ei;φi ∈ [e]; [φ], EWP[ι] eval η ei @ E <|Ψ|> {{ φi }}).
   Proof. iIntros "He". simpl. iFrame. Qed.
 
   Lemma ewp_ETuple η es φs φ E Ψ :
-    ([∗ list] ei; φi ∈ es; φs, EWP eval η ei @ E <|Ψ|> {{ ensures v, φi v }}) -∗
+    ([∗ list] ei; φi ∈ es; φs, EWP[ι] eval η ei @ E <|Ψ|> {{ ensures v, φi v }}) -∗
     (∀ vs, ([∗ list] vi; φi ∈ vs; φs, φi vi) -∗ φ (VTuple vs)) -∗
-    EWP eval η (ETuple es) @ E <|Ψ|> {{ ensures vs, φ vs }}.
+    EWP[ι] eval η (ETuple es) @ E <|Ψ|> {{ ensures vs, φ vs }}.
   Proof.
     iIntros "H P".
     iApply (ewp_mono_ret with "[H]").
@@ -328,24 +295,24 @@ Section ewp_rules_expr.
 
   Lemma ewp_EUnit_exn η φ E Ψ :
     φ (O2Ret VUnit) -∗
-    EWP eval η EUnit @ E <|Ψ|> {{ φ }}.
+    EWP[ι]eval η EUnit @ E <|Ψ|> {{ φ }}.
   Proof.
     simpl_eval; iApply ewp_ret.
   Qed.
 
   Lemma ewp_EUnit_forward η E Ψ :
-    ⊢ EWP eval η EUnit @ E <|Ψ|> {{ RET= #() }}.
+    ⊢ EWP[ι] eval η EUnit @ E <|Ψ|> {{ RET= #() }}.
   Proof.
     simpl_eval; by iApply ewp_ret.
   Qed.
 
   Lemma ewp_EPair_exn η e1 e2 (φ1 φ2 φ : outcome2 val exn -> _) E Ψ :
-    EWP eval η e1 @ E <|Ψ|> {{ φ1 }} -∗
-    EWP eval η e2 @ E <|Ψ|> {{ φ2 }} -∗
+    EWP[ι] eval η e1 @ E <|Ψ|> {{ φ1 }} -∗
+    EWP[ι] eval η e2 @ E <|Ψ|> {{ φ2 }} -∗
     (∀ v1 v2, φ1 (O2Ret v1) -∗ φ2 (O2Ret v2) -∗ φ (O2Ret (#(v1, v2)))) -∗
     (∀ e, φ1 (O2Throw e) -∗ φ (O2Throw e)) -∗
     (∀ e, φ2 (O2Throw e) -∗ φ (O2Throw e)) -∗
-    EWP eval η (EPair e1 e2) @ E <|Ψ|> {{ φ }}.
+    EWP[ι] eval η (EPair e1 e2) @ E <|Ψ|> {{ φ }}.
   Proof.
     iIntros "H1 H2 P E1 E2".
     iApply (ewp_ETuple_exn _ _ [φ1; φ2] with "[H1 H2] [P]").
@@ -356,19 +323,19 @@ Section ewp_rules_expr.
   Qed.
 
   Lemma ewp_EPair_ret η e1 e2 φ1 φ2 E Ψ φ :
-    EWP eval η e1 @ E <|Ψ|> {{ ensures v, φ1 v }} -∗
-    EWP eval η e2 @ E <|Ψ|> {{ ensures v, φ2 v }} -∗
+    EWP[ι] eval η e1 @ E <|Ψ|> {{ ensures v, φ1 v }} -∗
+    EWP[ι] eval η e2 @ E <|Ψ|> {{ ensures v, φ2 v }} -∗
     (∀ v1 v2, φ1 v1 -∗ φ2 v2 -∗ φ #(v1, v2)) -∗
-    EWP eval η (EPair e1 e2) @ E <|Ψ|> {{ ensures v, φ v }}.
+    EWP[ι] eval η (EPair e1 e2) @ E <|Ψ|> {{ ensures v, φ v }}.
   Proof.
     iIntros "H1 H2 P".
     iApply (ewp_EPair_exn with "H1 H2 [P]"); auto.
   Qed.
 
   Lemma ewp_EPair_ret_encode η e1 e2 `{Encode A} `{Encode B} (v1 : A) (v2 : B) R1 R2 E Ψ :
-    EWP eval η e1 @ E <|Ψ|> {{ ensures #r, ⌜r = v1⌝ ∗ R1 }} -∗
-    EWP eval η e2 @ E <|Ψ|> {{ ensures #r, ⌜r = v2⌝ ∗ R2 }} -∗
-    EWP eval η (EPair e1 e2) @ E <|Ψ|> {{ ensures #r, ⌜r = (v1, v2)⌝ ∗ R1 ∗ R2 }}.
+    EWP[ι] eval η e1 @ E <|Ψ|> {{ ensures #r, ⌜r = v1⌝ ∗ R1 }} -∗
+    EWP[ι] eval η e2 @ E <|Ψ|> {{ ensures #r, ⌜r = v2⌝ ∗ R2 }} -∗
+    EWP[ι] eval η (EPair e1 e2) @ E <|Ψ|> {{ ensures #r, ⌜r = (v1, v2)⌝ ∗ R1 ∗ R2 }}.
   Proof.
     iIntros "H1 H2".
     iApply (ewp_mono_ret with "[H1 H2]").
@@ -386,9 +353,9 @@ Section ewp_rules_expr.
   Qed.
 
   Lemma ewp_EPair_forward η e1 e2 `{Encode A} `{Encode B} (v1 : A) (v2 : B) R1 R2 E Ψ :
-    EWP eval η e1 @ E <|Ψ|> {{ RET= #v1, R1 }} -∗
-    EWP eval η e2 @ E <|Ψ|> {{ RET= #v2, R2 }} -∗
-    EWP eval η (EPair e1 e2) @ E <|Ψ|> {{ RET= #(v1, v2), R1 ∗ R2 }}.
+    EWP[ι] eval η e1 @ E <|Ψ|> {{ RET= #v1, R1 }} -∗
+    EWP[ι] eval η e2 @ E <|Ψ|> {{ RET= #v2, R2 }} -∗
+    EWP[ι] eval η (EPair e1 e2) @ E <|Ψ|> {{ RET= #(v1, v2), R1 ∗ R2 }}.
   Proof.
     iIntros "H1 H2".
     iApply (ewp_mono_ret with "[-]"). iApply (ewp_EPair_ret_encode with "[H1] [H2]").
@@ -410,13 +377,13 @@ Section ewp_rules_expr.
     (∀ a, φ1 (O2Ret a) -∗ φ2 (O2Ret (f a)))%I.
 
   Lemma ewp_EData_exn η c es E ψ φs φ :
-    ([∗ list] ei;φi ∈ es;φs, EWP eval η ei @ E <|ψ|> {{ φi }}) -∗
+    ([∗ list] ei;φi ∈ es;φs, EWP[ι] eval η ei @ E <|ψ|> {{ φi }}) -∗
     (∀ vs, ([∗ list] vi;φi ∈ vs;φs, φi (O2Ret vi)) -∗ φ (O2Ret (VData c vs))) -∗
     ([∗ list] φi ∈ φs, ∀ e, φi (O2Throw e) -∗ φ (O2Throw e)) -∗
-    EWP eval η (EData c es) @ E <|ψ|> {{ φ }}.
+    EWP[ι] eval η (EData c es) @ E <|ψ|> {{ φ }}.
   Proof.
     iIntros "H P E /=". simpl_eval.
-    iApply ewp_bind_exn.
+    iApply ewp_bind'.
     iApply (ewp_mono with "[H E]"); first iApply ewp_evals.
     - iPoseProof (big_sepL2_length with "[$]") as "%".
       setoid_rewrite big_sepL2_fmap_r.
@@ -436,11 +403,12 @@ Section ewp_rules_expr.
   Qed.
 
   Lemma ewp_EData η c es E ψ φs φ :
-    ([∗ list] ei;φi ∈ es;φs, EWP eval η ei @ E <| ψ |> {{ ensures v, φi v }}) -∗
+    ([∗ list] ei;φi ∈ es;φs, EWP[ι] eval η ei @ E <| ψ |> {{ ensures v, φi v }}) -∗
     (∀ vs : list val, ([∗ list] vi;φi ∈ vs;φs, φi vi) -∗ φ (VData c vs)) -∗
-    EWP eval η (EData c es) @ E <|ψ|> {{ ensures v, φ v }}.
+    EWP[ι] eval η (EData c es) @ E <|ψ|> {{ ensures v, φ v }}.
   Proof.
-    iIntros "Hes Hmon /=". simpl_eval.
+    iIntros "Hes Hmon /=".
+    simpl_eval.
     iApply ewp_bind.
     replace ('vs ← evals η es; ret (VTuple vs)) with (eval η (ETuple es)); last first.
     { simpl_eval; reflexivity. }
@@ -453,7 +421,7 @@ Section ewp_rules_expr.
   (* E/VConstant is a macro for E/VData *)
   Lemma ewp_EConstant η c E Ψ φ :
     φ (O2Ret (VConstant c)) -∗
-    EWP eval η (EConstant c) @ E <|Ψ|> {{ φ }}.
+    EWP[ι] eval η (EConstant c) @ E <|Ψ|> {{ φ }}.
   Proof.
     iIntros "H". simpl_eval. by iApply ewp_ret.
   Qed.
@@ -461,14 +429,14 @@ Section ewp_rules_expr.
   (** * EXData : data → expr → expr *)
   Lemma ewp_EXData_exn η π l e E ψ φ1 φ :
     lookup_path η π = ret (VLoc l) ->
-    EWP evals η e @ E <|ψ|> {{ φ1 }} -∗
+    EWP[ι] evals η e @ E <|ψ|> {{ φ1 }} -∗
     propagate_exn φ1 φ -∗
     propagate_ret_fmap (λ v : list val, VXData l v) φ1 φ -∗
-    EWP eval η (EXData π e) @ E <|ψ|> {{ φ }}.
+    EWP[ι] eval η (EXData π e) @ E <|ψ|> {{ φ }}.
   Proof.
     iIntros (Hlookup) "He Hexn Hret".
     simpl_eval. rewrite Hlookup. simpl.
-    iApply ewp_bind_exn.
+    iApply ewp_bind'.
     iApply (ewp_mono with "He").
     iIntros ([|]) "Hφ".
     - iApply ewp_ret. by iApply "Hret".
@@ -477,9 +445,9 @@ Section ewp_rules_expr.
 
   Lemma ewp_EXData η π l es E ψ φs φ :
     lookup_path η π = ret (VLoc l) ->
-    ([∗ list] ei;φi ∈ es;φs, EWP eval η ei @ E <| ψ |> {{ ensures v, φi v }}) -∗
+    ([∗ list] ei;φi ∈ es;φs, EWP[ι]eval η ei @ E <| ψ |> {{ ensures v, φi v }}) -∗
     (∀ vs : list val, ([∗ list] vi;φi ∈ vs;φs, φi vi) -∗ φ (VXData l vs)) -∗
-    EWP eval η (EXData π es) @ E <|ψ|> {{ ensures v, φ v }}.
+    EWP[ι]eval η (EXData π es) @ E <|ψ|> {{ ensures v, φ v }}.
   Proof.
     iIntros (Hlookup) "He Hmon".
     simpl_eval. rewrite Hlookup. simpl.
@@ -501,14 +469,14 @@ Section ewp_rules_expr.
   (** * EInt : Z → expr *)
 
   Lemma ewp_EInt_forward η i E Ψ :
-    ⊢ EWP eval η (EInt i) @ E <|Ψ|> {{ RET= #i }}.
+    ⊢ EWP[ι]eval η (EInt i) @ E <|Ψ|> {{ RET= #i }}.
   Proof.
     simpl_eval; by iApply ewp_ret.
   Qed.
 
   Lemma ewp_EInt η i φ E Ψ :
     φ (O2Ret #i) -∗
-    EWP eval η (EInt i) @ E <|Ψ|> {{ φ }}.
+    EWP[ι]eval η (EInt i) @ E <|Ψ|> {{ φ }}.
   Proof.
     simpl_eval; by iApply ewp_ret.
   Qed.
@@ -518,7 +486,7 @@ Section ewp_rules_expr.
   (** * EIntNeg : expr → expr *)
   (** * EIntAdd : expr → expr → expr *)
 
-  Lemma ewpi_EIntAdd_exn ι η e1 e2 φ1 φ2 φ E Ψ :
+  Lemma ewp_EIntAdd_exn η e1 e2 φ1 φ2 φ E Ψ :
     EWP[ι] as_int (eval η e1) @ E <|Ψ|> {{ φ1 }} -∗
     EWP[ι] as_int (eval η e2) @ E <|Ψ|> {{ φ2 }} -∗
     (∀ v, φ1 (O2Throw v) -∗ φ (O2Throw v)) -∗
@@ -527,24 +495,24 @@ Section ewp_rules_expr.
     EWP[ι] eval η (EIntAdd e1 e2) @ E <|Ψ|> {{ φ }}.
   Proof.
     iIntros "H1 H2 E1 E2 P /=". simpl_eval.
-    iApply (ewpi_Par with "H1 H2 [E1] [E2]").
-    - iIntros (v) "H /=". iApply ewpi_throw. iApply ("E1" with "H").
-    - iIntros (v) "H /=". iApply ewpi_throw. iApply ("E2" with "H").
-    - iIntros (n1 n2) "H1 H2". iApply ewpi_bind. iApply ewpi_ret. iApply ewpi_ret.
+    iApply (ewp_Par with "H1 H2 [E1] [E2]").
+    - iIntros (v) "H /=". iApply ewp_throw. iApply ("E1" with "H").
+    - iIntros (v) "H /=". iApply ewp_throw. iApply ("E2" with "H").
+    - iIntros (n1 n2) "H1 H2". iApply ewp_bind. iApply ewp_ret. iApply ewp_ret.
       iApply "P". iFrame.
   Qed.
 
-  Lemma ewpi_EIntAdd ι η e1 e2 φ1 φ2 φ E Ψ :
+  Lemma ewp_EIntAdd η e1 e2 φ1 φ2 φ E Ψ :
     EWP[ι] as_int (eval η e1) @ E <|Ψ|> {{ ensures n1, φ1 n1 }} -∗
     EWP[ι] as_int (eval η e2) @ E <|Ψ|> {{ ensures n2, φ2 n2 }} -∗
     (∀ n1 n2, φ1 n1 ∗ φ2 n2 -∗ φ (VInt (int.M.add n1 n2))) -∗
     EWP[ι] eval η (EIntAdd e1 e2) @ E <|Ψ|> {{ ensures n, φ n }}.
   Proof.
     iIntros "H1 H2 P".
-    iApply (ewpi_EIntAdd_exn with "H1 H2"); auto.
+    iApply (ewp_EIntAdd_exn with "H1 H2"); auto.
   Qed.
 
-  Lemma ewpi_EIntAdd' ι η e1 e2 (φ1 φ2 φ : Z -> iProp Σ) E Ψ :
+  Lemma ewp_EIntAdd' η e1 e2 (φ1 φ2 φ : Z -> iProp Σ) E Ψ :
     EWP[ι] eval η e1 @ E <|Ψ|> {{ ensures #n1, φ1 n1 }} -∗
     EWP[ι] eval η e2 @ E <|Ψ|> {{ ensures #n2, φ2 n2 }} -∗
     (∀ n1 n2, φ1 n1 ∗ φ2 n2 -∗ φ (n1 + n2)%Z) -∗
@@ -553,15 +521,15 @@ Section ewp_rules_expr.
     iIntros "H1 H2 P".
     pose φ1' := (λ v, ∃ n, ⌜v = repr n⌝∗ φ1 n)%I.
     pose φ2' := (λ v, ∃ n, ⌜v = repr n⌝∗ φ2 n)%I.
-    iApply (ewpi_EIntAdd ι _ _ _ φ1' φ2' with "[H1] [H2]"); auto.
-    - iApply ewpi_bind. iApply (ewpi_mono with "H1").
+    iApply (ewp_EIntAdd _ _ _ φ1' φ2' with "[H1] [H2]"); auto.
+    - iApply ewp_bind. iApply (ewp_mono with "H1").
       iIntros ([|]); [ | iIntros ([]) ].
       iIntros "(%n & -> & H)".
-      iApply ewpi_ret. iExists _. by iFrame.
-    - iApply ewpi_bind. iApply (ewpi_mono with "H2").
+      iApply ewp_ret. iExists _. by iFrame.
+    - iApply ewp_bind. iApply (ewp_mono with "H2").
       iIntros ([|]); [ | iIntros ([]) ].
       iIntros "(%n & -> & H)".
-      iApply ewpi_ret. iExists _. by iFrame.
+      iApply ewp_ret. iExists _. by iFrame.
     - iIntros (i1 i2) "(H1 & H2)".
       iDestruct "H1" as (n1 ->) "H1".
       iDestruct "H2" as (n2 ->) "H2".
@@ -570,42 +538,10 @@ Section ewp_rules_expr.
       rewrite M.add_repr_repr. auto.
   Qed.
 
-  Lemma ewp_EIntAdd_exn η e1 e2 φ1 φ2 φ E Ψ :
-    EWP as_int (eval η e1) @ E <|Ψ|> {{ φ1 }} -∗
-    EWP as_int (eval η e2) @ E <|Ψ|> {{ φ2 }} -∗
-    (∀ v, φ1 (O2Throw v) -∗ φ (O2Throw v)) -∗
-    (∀ v, φ2 (O2Throw v) -∗ φ (O2Throw v)) -∗
-    (∀ n1 n2, φ1 (O2Ret n1) ∗ φ2 (O2Ret n2) -∗ φ (O2Ret (VInt (int.M.add n1 n2)))) -∗
-    EWP eval η (EIntAdd e1 e2) @ E <|Ψ|> {{ φ }}.
-  Proof.
-    iIntros "H1 H2 E1 E2 P /= %ι".
-    iApply (ewpi_EIntAdd_exn with "H1 H2 E1 E2 P").
-  Qed.
-
-  Lemma ewp_EIntAdd η e1 e2 φ1 φ2 φ E Ψ :
-    EWP as_int (eval η e1) @ E <|Ψ|> {{ ensures n1, φ1 n1 }} -∗
-    EWP as_int (eval η e2) @ E <|Ψ|> {{ ensures n2, φ2 n2 }} -∗
-    (∀ n1 n2, φ1 n1 ∗ φ2 n2 -∗ φ (VInt (int.M.add n1 n2))) -∗
-    EWP eval η (EIntAdd e1 e2) @ E <|Ψ|> {{ ensures n, φ n }}.
-  Proof.
-    iIntros "H1 H2 P".
-    iApply (ewp_EIntAdd_exn with "H1 H2"); auto.
-  Qed.
-
-  Lemma ewp_EIntAdd' η e1 e2 (φ1 φ2 φ : Z -> iProp Σ) E Ψ :
-    EWP eval η e1 @ E <|Ψ|> {{ ensures #n1, φ1 n1 }} -∗
-    EWP eval η e2 @ E <|Ψ|> {{ ensures #n2, φ2 n2 }} -∗
-    (∀ n1 n2, φ1 n1 ∗ φ2 n2 -∗ φ (n1 + n2)%Z) -∗
-    EWP eval η (EIntAdd e1 e2) @ E <|Ψ|> {{ ensures #n, φ n }}.
-  Proof.
-    iIntros "H1 H2 P %ι".
-    iApply (ewpi_EIntAdd' with "H1 H2 P").
-  Qed.
-
   Lemma ewp_EIntAdd_simple η e1 e2 (n1 n2 : Z) (R1 R2 : iProp Σ) E Ψ :
-    EWP eval η e1 @ E <|Ψ|> {{ RET= #n1, R1 }} -∗
-    EWP eval η e2 @ E <|Ψ|> {{ RET= #n2, R2 }} -∗
-    EWP eval η (EIntAdd e1 e2) @ E <|Ψ|> {{ RET= #(n1 + n2)%Z, R1 ∗ R2 }}.
+    EWP[ι] eval η e1 @ E <|Ψ|> {{ RET= #n1, R1 }} -∗
+    EWP[ι] eval η e2 @ E <|Ψ|> {{ RET= #n2, R2 }} -∗
+    EWP[ι] eval η (EIntAdd e1 e2) @ E <|Ψ|> {{ RET= #(n1 + n2)%Z, R1 ∗ R2 }}.
   Proof.
     iIntros "H1 H2".
     iApply (ewp_EIntAdd _ _ _
@@ -637,13 +573,13 @@ Section ewp_rules_expr.
   (** * EOpEq : expr → expr → expr *)
 
   Lemma ewp_EOpEq_exn η e1 e2 φ1 φ2 φ E Ψ :
-    EWP eval η e1 @ E <|Ψ|> {{ φ1 }} -∗
-    EWP eval η e2 @ E <|Ψ|> {{ φ2 }} -∗
+    EWP[ι]eval η e1 @ E <|Ψ|> {{ φ1 }} -∗
+    EWP[ι]eval η e2 @ E <|Ψ|> {{ φ2 }} -∗
     (∀ v, φ1 (O2Throw v) -∗ φ (O2Throw v)) -∗
     (∀ v, φ2 (O2Throw v) -∗ φ (O2Throw v)) -∗
     (∀ v1 v2, φ1 (O2Ret v1) ∗ φ2 (O2Ret v2) -∗
-      EWP eq_val v1 v2 @ E <|Ψ|> {{ ensures b, φ (O2Ret (VBool b)) }}) -∗
-    EWP eval η (EOpEq e1 e2) @ E <|Ψ|> {{ φ }}.
+      EWP[ι]eq_val v1 v2 @ E <|Ψ|> {{ ensures b, φ (O2Ret (VBool b)) }}) -∗
+    EWP[ι]eval η (EOpEq e1 e2) @ E <|Ψ|> {{ φ }}.
   Proof.
     iIntros "H1 H2 E1 E2 P /=". simpl_eval.
     iApply (ewp_Par with "H1 H2 [E1] [E2]").
@@ -659,11 +595,11 @@ Section ewp_rules_expr.
 
   Lemma ewp_EOpEq η e1 e2 (φ1 φ2 : val -> iProp Σ)
     (φ : outcome2 val exn -> iProp Σ) E Ψ :
-    EWP eval η e1 @ E <|Ψ|> {{ ensures v1, φ1 v1 }} -∗
-    EWP eval η e2 @ E <|Ψ|> {{ ensures v2, φ2 v2 }} -∗
+    EWP[ι]eval η e1 @ E <|Ψ|> {{ ensures v1, φ1 v1 }} -∗
+    EWP[ι]eval η e2 @ E <|Ψ|> {{ ensures v2, φ2 v2 }} -∗
     (∀ v1 v2, φ1 v1 ∗ φ2 v2 -∗
-      EWP eq_val v1 v2 @ E <|Ψ|> {{ ensures b, φ (O2Ret (VBool b)) }}) -∗
-    EWP eval η (EOpEq e1 e2) @ E <|Ψ|> {{ φ }}.
+      EWP[ι]eq_val v1 v2 @ E <|Ψ|> {{ ensures b, φ (O2Ret (VBool b)) }}) -∗
+    EWP[ι]eval η (EOpEq e1 e2) @ E <|Ψ|> {{ φ }}.
   Proof.
     iIntros "H1 H2 P".
     iApply (ewp_EOpEq_exn with "H1 H2"); auto.
@@ -673,9 +609,9 @@ Section ewp_rules_expr.
   Lemma ewp_EOpEq_simple_Z η e1 e2 (n1 n2 : Z) (R1 R2 : iProp Σ) E Ψ :
     representable n1 ->
     representable n2 ->
-    EWP eval η e1 @ E <|Ψ|> {{ RET= #n1, R1 }} -∗
-    EWP eval η e2 @ E <|Ψ|> {{ RET= #n2, R2 }} -∗
-    EWP eval η (EOpEq e1 e2) @ E <|Ψ|> {{ RET= #(n1 =? n2)%Z, R1 ∗ R2 }}.
+    EWP[ι]eval η e1 @ E <|Ψ|> {{ RET= #n1, R1 }} -∗
+    EWP[ι]eval η e2 @ E <|Ψ|> {{ RET= #n2, R2 }} -∗
+    EWP[ι]eval η (EOpEq e1 e2) @ E <|Ψ|> {{ RET= #(n1 =? n2)%Z, R1 ∗ R2 }}.
   Proof.
     iIntros (Hn1 Hn2) "H1 H2".
     iApply (ewp_EOpEq _ _ _
@@ -698,13 +634,13 @@ Section ewp_rules_expr.
 
   (* Intermediate lemma: using [eval_bindings] hypothesis *)
   Lemma ewp_ELet_exn η bs e φ1 φ E Ψ :
-    EWP eval_bindings η bs @ E <|Ψ|> {{ φ1 }} -∗
+    EWP[ι] eval_bindings η bs @ E <|Ψ|> {{ φ1 }} -∗
     (∀ v, φ1 (O2Throw v) -∗ φ (O2Throw v)) -∗
-    (∀ δ, φ1 (O2Ret δ) -∗ EWP eval (δ ++ η) e @ E <|Ψ|> {{ φ }}) -∗
-    EWP eval η (ELet bs e) @ E <|Ψ|> {{ φ }}.
+    (∀ δ, φ1 (O2Ret δ) -∗ EWP[ι] eval (δ ++ η) e @ E <|Ψ|> {{ φ }}) -∗
+    EWP[ι] eval η (ELet bs e) @ E <|Ψ|> {{ φ }}.
   Proof.
     iIntros "Hη E P /=". simpl_eval.
-    iApply ewp_bind_exn.
+    iApply ewp_bind'.
     iApply (ewp_mono with "Hη").
     iIntros ([δ|v]) "H/=".
     - iApply ("P" with "H").
@@ -712,9 +648,9 @@ Section ewp_rules_expr.
   Qed.
 
   Lemma ewp_ELet {η bs e} (φ' : env -> iProp Σ) φ E Ψ :
-    EWP eval_bindings η bs @ E <|Ψ|> {{ ensures v, φ' v }} -∗
-    (∀ δ, φ' δ -∗ EWP eval (δ ++ η) e @ E <|Ψ|> {{ φ }}) -∗
-    EWP eval η (ELet bs e) @ E <|Ψ|> {{ φ }}.
+    EWP[ι] eval_bindings η bs @ E <|Ψ|> {{ ensures v, φ' v }} -∗
+    (∀ δ, φ' δ -∗ EWP[ι] eval (δ ++ η) e @ E <|Ψ|> {{ φ }}) -∗
+    EWP[ι] eval η (ELet bs e) @ E <|Ψ|> {{ φ }}.
   Proof.
     iIntros "Hη P /=". simpl_eval.
     iApply ewp_bind.
@@ -727,14 +663,14 @@ Section ewp_rules_expr.
 
   (* TODO: Have *_singleton *_cons lemmas about relevant expr constructs *)
   Corollary ewp_ELet_singleton_total {η p e e'} (Φ : val -> iProp Σ) φ φ' E Ψ:
-    EWP eval η e' @ E <|Ψ|> {{ ensures v, Φ v }} -∗
+    EWP[ι] eval η e' @ E <|Ψ|> {{ ensures v, Φ v }} -∗
     (∀ v, Φ v -∗ ⌜pure_wp (irrefutably_extend η nil p v) (φ v) ⊥⌝) -∗
     (∀ v δ, Φ v -∗ ⌜φ v δ⌝ -∗
-            EWP eval (δ ++ η) e @ E <|Ψ|> {{ φ' }}) -∗
-    EWP eval η (ELet [ Binding p e' ] e) @ E <|Ψ|> {{ φ' }}.
+            EWP[ι] eval (δ ++ η) e @ E <|Ψ|> {{ φ' }}) -∗
+    EWP[ι] eval η (ELet [ Binding p e' ] e) @ E <|Ψ|> {{ φ' }}.
   Proof.
     iIntros "He' HP He".
-    iApply (ewp_ELet (λ δ, EWP eval (δ ++ η) e @ E <|Ψ|> {{ φ' }})%I
+    iApply (ewp_ELet (λ δ, EWP[ι]eval (δ ++ η) e @ E <|Ψ|> {{ φ' }})%I
       with "[He' HP He]").
     { iApply (ewp_eval_bindings_singleton_total with "He' HP").
       iIntros (v δ) "HΦ Hφ".
@@ -744,9 +680,9 @@ Section ewp_rules_expr.
 
   (* Special case of [let x = e' in e] *)
   Lemma ewp_ELet_PVar_1 {η x e e'} (Φ : val -> iProp Σ) φ E Ψ:
-    EWP eval η e' @ E <|Ψ|> {{ ensures v, Φ v }} -∗
-    (∀ v, Φ v -∗ EWP eval ((x, v) :: η) e @ E <|Ψ|> {{ φ }}) -∗
-    EWP eval η (ELet [Binding (PVar x) e'] e) @ E <|Ψ|> {{ φ }}.
+    EWP[ι]eval η e' @ E <|Ψ|> {{ ensures v, Φ v }} -∗
+    (∀ v, Φ v -∗ EWP[ι]eval ((x, v) :: η) e @ E <|Ψ|> {{ φ }}) -∗
+    EWP[ι]eval η (ELet [Binding (PVar x) e'] e) @ E <|Ψ|> {{ φ }}.
   Proof.
     iIntros "H P".
     iApply (ewp_ELet_singleton_total with "H").
@@ -760,9 +696,9 @@ Section ewp_rules_expr.
 
   (* Alternative form *)
   Lemma ewp_ELet_PVar_1_forward {η x e e' v} R φ E Ψ:
-    EWP eval η e' @ E <|Ψ|> {{ RET= v, R }} -∗
-    (R -∗ EWP eval ((x, v) :: η) e @ E <|Ψ|> {{ φ }}) -∗
-    EWP eval η (ELet [ Binding (PVar x) e' ] e) @ E <|Ψ|> {{ φ }}.
+    EWP[ι]eval η e' @ E <|Ψ|> {{ RET= v, R }} -∗
+    (R -∗ EWP[ι]eval ((x, v) :: η) e @ E <|Ψ|> {{ φ }}) -∗
+    EWP[ι]eval η (ELet [ Binding (PVar x) e' ] e) @ E <|Ψ|> {{ φ }}.
   Proof.
     iIntros "H P".
     iApply (ewp_ELet_PVar_1 with "H").
@@ -772,9 +708,9 @@ Section ewp_rules_expr.
 
   (* Special case of [let _ = e' in e] *)
   Lemma ewp_ELet_PAny_1 {η e e'} R φ E Ψ:
-    EWP eval η e' @ E <|Ψ|> {{ ensures _, R }} -∗
-    (R -∗ EWP eval η e @ E <|Ψ|> {{ φ }}) -∗
-    EWP eval η (ELet [Binding PAny e'] e) @ E <|Ψ|> {{ φ }}.
+    EWP[ι]eval η e' @ E <|Ψ|> {{ ensures _, R }} -∗
+    (R -∗ EWP[ι]eval η e @ E <|Ψ|> {{ φ }}) -∗
+    EWP[ι]eval η (ELet [Binding PAny e'] e) @ E <|Ψ|> {{ φ }}.
   Proof.
     iIntros "H P".
     iApply (ewp_ELet_singleton_total with "H").
@@ -790,8 +726,8 @@ Section ewp_rules_expr.
 
   Lemma ewp_ELetRec η bs e φ E Ψ :
     let δ := eval_rec_bindings η bs in
-    EWP eval (δ ++ η) e @ E <|Ψ|> {{ φ }} -∗
-    EWP eval η (ELetRec bs e) @ E <|Ψ|> {{ φ }}.
+    EWP[ι]eval (δ ++ η) e @ E <|Ψ|> {{ φ }} -∗
+    EWP[ι]eval η (ELetRec bs e) @ E <|Ψ|> {{ φ }}.
   Proof.
     simpl_eval; auto.
   Qed.
@@ -802,12 +738,12 @@ Section ewp_rules_expr.
   variable *)
   Lemma ewp_ELetRec_specced_1 {η f x e1 e2 φ E Ψ} {A : Type} (R : A → val → iProp Σ) φf :
     □(∀ vf,
-     □(∀ a v, R a v -∗ EWP call vf v <|Ψ|> {{ φf a }}) -∗
-       ∀ a v, R a v -∗ EWP eval ((x, v) :: (f, vf) :: η) e1 <|Ψ|> {{ φf a }}) -∗
+     □(∀ a v, R a v -∗ EWP[ι]call vf v <|Ψ|> {{ φf a }}) -∗
+       ∀ a v, R a v -∗ EWP[ι]eval ((x, v) :: (f, vf) :: η) e1 <|Ψ|> {{ φf a }}) -∗
     (∀ vf,
-      □(∀ a v, R a v -∗ EWP call vf v <|Ψ|> {{ φf a }}) -∗
-      EWP eval ((f, vf) :: η) e2 @ E <|Ψ|> {{ φ }}) -∗
-    EWP eval η (ELetRec [RecBinding f (AnonFun x e1)] e2) @ E <|Ψ|> {{ φ }}.
+      □(∀ a v, R a v -∗ EWP[ι]call vf v <|Ψ|> {{ φf a }}) -∗
+      EWP[ι]eval ((f, vf) :: η) e2 @ E <|Ψ|> {{ φ }}) -∗
+    EWP[ι]eval η (ELetRec [RecBinding f (AnonFun x e1)] e2) @ E <|Ψ|> {{ φ }}.
   Proof.
     iIntros "#He1 He2".
     iApply ewp_ELetRec. simpl.
@@ -824,12 +760,12 @@ Section ewp_rules_expr.
 
   Lemma ewp_ELetRec_specced_ret_1 {η f x e1 e2 φ E Ψ} {A} (R : A → val → iProp Σ) φf :
     □(∀ vf,
-     □(∀ a v, R a v -∗ EWP call vf v <|Ψ|> {{ ensures v', φf a v' }}) -∗
-       ∀ a v, R a v -∗ EWP eval ((x, v) :: (f, vf) :: η) e1 <|Ψ|> {{ ensures v', φf a v' }}) -∗
+     □(∀ a v, R a v -∗ EWP[ι]call vf v <|Ψ|> {{ ensures v', φf a v' }}) -∗
+       ∀ a v, R a v -∗ EWP[ι]eval ((x, v) :: (f, vf) :: η) e1 <|Ψ|> {{ ensures v', φf a v' }}) -∗
     (∀ vf,
-      □(∀ a v, R a v -∗ EWP call vf v <|Ψ|> {{ ensures v', φf a v' }}) -∗
-      EWP eval ((f, vf) :: η) e2 @ E <|Ψ|> {{ φ }}) -∗
-    EWP eval η (ELetRec [RecBinding f (AnonFun x e1)] e2) @ E <|Ψ|> {{ φ }}.
+      □(∀ a v, R a v -∗ EWP[ι]call vf v <|Ψ|> {{ ensures v', φf a v' }}) -∗
+      EWP[ι]eval ((f, vf) :: η) e2 @ E <|Ψ|> {{ φ }}) -∗
+    EWP[ι]eval η (ELetRec [RecBinding f (AnonFun x e1)] e2) @ E <|Ψ|> {{ φ }}.
   Proof.
     iApply ewp_ELetRec_specced_1.
   Qed.
@@ -838,9 +774,9 @@ Section ewp_rules_expr.
 
   (** * ELetOpen : mexpr → expr → expr *)
   Lemma ewp_ELetOpen η me e E ψ φ :
-    EWP eval_mexpr η me @ E <|ψ|> {{ ensures m, ∃ δ, ⌜ m = VStruct δ ⌝ ∗
-    EWP eval (δ ++ η) e @ E <|ψ|> {{ φ }} }} -∗
-    EWP eval η (ELetOpen me e) @ E <|ψ|> {{ φ }}.
+    EWP[ι]eval_mexpr η me @ E <|ψ|> {{ ensures m, ∃ δ, ⌜ m = VStruct δ ⌝ ∗
+    EWP[ι]eval (δ ++ η) e @ E <|ψ|> {{ φ }} }} -∗
+    EWP[ι]eval η (ELetOpen me e) @ E <|ψ|> {{ φ }}.
   Proof.
     iIntros "Hme". simpl_eval.
     iApply ewp_bind.
@@ -855,13 +791,13 @@ Section ewp_rules_expr.
   (** * ESeq : expr → expr → expr *)
 
   Lemma ewp_ESeq_exn η e1 e2 φ1 φ E Ψ :
-    EWP eval η e1 @ E <|Ψ|> {{ φ1 }} -∗
+    EWP[ι]eval η e1 @ E <|Ψ|> {{ φ1 }} -∗
     (∀ v, φ1 (O2Throw v) -∗ φ (O2Throw v)) -∗
-    (∀ v1, φ1 (O2Ret v1) -∗ EWP eval η e2 @ E <|Ψ|> {{ φ }}) -∗
-    EWP eval η (ESeq e1 e2) @ E <|Ψ|> {{ φ }}.
+    (∀ v1, φ1 (O2Ret v1) -∗ EWP[ι]eval η e2 @ E <|Ψ|> {{ φ }}) -∗
+    EWP[ι]eval η (ESeq e1 e2) @ E <|Ψ|> {{ φ }}.
   Proof.
     iIntros "H M P /=". simpl_eval.
-    iApply ewp_bind_exn.
+    iApply ewp_bind'.
     iApply (ewp_mono with "H").
     iIntros ([v|v]) "/= H1".
     - iApply ("P" with "H1").
@@ -869,32 +805,25 @@ Section ewp_rules_expr.
   Qed.
 
   Lemma ewp_ESeq η e1 e2 φ E Ψ :
-    EWP eval η e1 @ E <|Ψ|> {{ ensures _, EWP eval η e2 @ E <|Ψ|> {{ φ }} }} -∗
-    EWP eval η (ESeq e1 e2) @ E <|Ψ|> {{ φ }}.
+    EWP[ι]eval η e1 @ E <|Ψ|> {{ ensures _, EWP[ι]eval η e2 @ E <|Ψ|> {{ φ }} }} -∗
+    EWP[ι]eval η (ESeq e1 e2) @ E <|Ψ|> {{ φ }}.
   Proof.
     iIntros "H". simpl_eval. by iApply ewp_bind.
-  Qed.
-
-  Lemma ewpi_ESeq ι η e1 e2 φ E Ψ :
-    EWP[ι] eval η e1 @ E <|Ψ|> {{ ensures _, EWP[ι] eval η e2 @ E <|Ψ|> {{ φ }} }} -∗
-    EWP[ι] eval η (ESeq e1 e2) @ E <|Ψ|> {{ φ }}.
-  Proof.
-    iIntros "H". simpl_eval. by iApply ewpi_bind.
   Qed.
 
   (** * EIfThen : expr → expr → expr *)
 
   Lemma ewp_EIfThen_exn' η eb e1 φb φ E Ψ :
-    EWP eval η eb @ E <|Ψ|> {{ φb }} -∗
+    EWP[ι] eval η eb @ E <|Ψ|> {{ φb }} -∗
     (∀ v, φb (O2Throw v) -∗ φ (O2Throw v)) -∗
     (∀ v, φb (O2Ret v) -∗
-      (⌜v = VTrue ⌝ ∗ EWP eval η e1 @ E <|Ψ|> {{ φ }})
+      (⌜v = VTrue ⌝ ∗ EWP[ι] eval η e1 @ E <|Ψ|> {{ φ }})
     ∨ (⌜v = VFalse⌝ ∗ φ (O2Ret VUnit))) -∗
-    EWP eval η (EIfThen eb e1) @ E <|Ψ|> {{ φ }}.
+    EWP[ι] eval η (EIfThen eb e1) @ E <|Ψ|> {{ φ }}.
   Proof.
     iIntros "Hb E P /=". simpl_eval.
-    iApply ewp_bind_exn.
-    iApply ewp_bind_exn.
+    iApply ewp_bind'.
+    iApply ewp_bind'.
     iApply (ewp_mono with "Hb"). iIntros ([v|v]) "H /=". 2: by iApply "E".
     iDestruct ("P" with "H") as "[(-> & H) | (-> & H)] /=";
       try assert (val_as_bool VTrue = ret true) as -> by reflexivity;
@@ -903,17 +832,17 @@ Section ewp_rules_expr.
   Qed.
 
   Lemma ewp_EIfThen_exn η eb e1 φb φ E Ψ :
-    EWP eval η eb @ E <|Ψ|> {{ φb }} -∗
+    EWP[ι]eval η eb @ E <|Ψ|> {{ φb }} -∗
     (∀ v, φb (O2Throw v) -∗ φ (O2Throw v)) -∗
     (∀ v, φb (O2Ret v) -∗
       ∃ b, ⌜v = VBool b⌝ ∗
-      if b then EWP eval η e1 @ E <|Ψ|> {{ φ }}
+      if b then EWP[ι]eval η e1 @ E <|Ψ|> {{ φ }}
            else φ (O2Ret VUnit)) -∗
-    EWP eval η (EIfThen eb e1) @ E <|Ψ|> {{ φ }}.
+    EWP[ι]eval η (EIfThen eb e1) @ E <|Ψ|> {{ φ }}.
   Proof.
     iIntros "Hb E P /=". simpl_eval.
-    iApply ewp_bind_exn.
-    iApply ewp_bind_exn.
+    iApply ewp_bind'.
+    iApply ewp_bind'.
     iApply (ewp_mono with "Hb"). iIntros ([v|v]) "H /=". 2: by iApply "E".
     iDestruct ("P" with "H") as ([]) "(-> & H) /=";
       try assert (val_as_bool VTrue = ret true) as -> by reflexivity;
@@ -922,10 +851,10 @@ Section ewp_rules_expr.
   Qed.
 
   Lemma ewp_EIfThen η eb e1 φ E Ψ :
-    EWP eval η eb @ E <|Ψ|> {{ ensures v,
-      (⌜v = VTrue ⌝ ∗ EWP eval η e1 @ E <|Ψ|> {{ φ }})
+    EWP[ι]eval η eb @ E <|Ψ|> {{ ensures v,
+      (⌜v = VTrue ⌝ ∗ EWP[ι]eval η e1 @ E <|Ψ|> {{ φ }})
     ∨ (⌜v = VFalse⌝ ∗ φ (O2Ret VUnit)) }} -∗
-    EWP eval η (EIfThen eb e1) @ E <|Ψ|> {{ φ }}.
+    EWP[ι]eval η (EIfThen eb e1) @ E <|Ψ|> {{ φ }}.
   Proof.
     iIntros "H".
     iApply (ewp_EIfThen_exn' with "H").
@@ -936,16 +865,16 @@ Section ewp_rules_expr.
   (** * EIfThenElse : expr → expr → expr → expr *)
 
   Lemma ewp_EIfThenElse_exn' η eb e1 e2 φb φ E Ψ :
-    EWP eval η eb @ E <|Ψ|> {{ φb }} -∗
+    EWP[ι] eval η eb @ E <|Ψ|> {{ φb }} -∗
     (∀ v, φb (O2Throw v) -∗ φ (O2Throw v)) -∗
     (∀ v, φb (O2Ret v) -∗
-      (⌜v = VTrue ⌝ ∗ EWP eval η e1 @ E <|Ψ|> {{ φ }})
-    ∨ (⌜v = VFalse⌝ ∗ EWP eval η e2 @ E <|Ψ|> {{ φ }})) -∗
-    EWP eval η (EIfThenElse eb e1 e2) @ E <|Ψ|> {{ φ }}.
+      (⌜v = VTrue ⌝ ∗ EWP[ι] eval η e1 @ E <|Ψ|> {{ φ }})
+    ∨ (⌜v = VFalse⌝ ∗ EWP[ι] eval η e2 @ E <|Ψ|> {{ φ }})) -∗
+    EWP[ι] eval η (EIfThenElse eb e1 e2) @ E <|Ψ|> {{ φ }}.
   Proof.
     iIntros "Hb E P /=". simpl_eval.
-    iApply ewp_bind_exn.
-    iApply ewp_bind_exn.
+    iApply ewp_bind'.
+    iApply ewp_bind'.
     iApply (ewp_mono with "Hb"). iIntros ([v|v]) "H /=". 2: by iApply "E".
     iDestruct ("P" with "H") as "[(-> & H) | (-> & H)] /=";
       try assert (val_as_bool VTrue = ret true) as -> by reflexivity;
@@ -954,17 +883,17 @@ Section ewp_rules_expr.
   Qed.
 
   Lemma ewp_EIfThenElse_exn η eb e1 e2 φb φ E Ψ :
-    EWP eval η eb @ E <|Ψ|> {{ φb }} -∗
+    EWP[ι] eval η eb @ E <|Ψ|> {{ φb }} -∗
     (∀ v, φb (O2Throw v) -∗ φ (O2Throw v)) -∗
     (∀ v, φb (O2Ret v) -∗
       ∃ b, ⌜v = VBool b⌝ ∗
-      if b then EWP eval η e1 @ E <|Ψ|> {{ φ }}
-           else EWP eval η e2 @ E <|Ψ|> {{ φ }}) -∗
-    EWP eval η (EIfThenElse eb e1 e2) @ E <|Ψ|> {{ φ }}.
+      if b then EWP[ι] eval η e1 @ E <|Ψ|> {{ φ }}
+           else EWP[ι] eval η e2 @ E <|Ψ|> {{ φ }}) -∗
+    EWP[ι] eval η (EIfThenElse eb e1 e2) @ E <|Ψ|> {{ φ }}.
   Proof.
     iIntros "Hb E P". simpl_eval.
-    iApply ewp_bind_exn.
-    iApply ewp_bind_exn.
+    iApply ewp_bind'.
+    iApply ewp_bind'.
     iApply (ewp_mono with "Hb"). iIntros ([v|v]) "H /=". 2: by iApply "E".
     iDestruct ("P" with "H") as ([]) "(-> & H) /=";
       try assert (val_as_bool VTrue = ret true) as -> by reflexivity;
@@ -973,10 +902,10 @@ Section ewp_rules_expr.
   Qed.
 
   Lemma ewp_EIfThenElse η eb e1 e2 φ E Ψ :
-    EWP eval η eb @ E <|Ψ|> {{ ensures v,
-      (⌜v = VTrue ⌝ ∗ EWP eval η e1 @ E <|Ψ|> {{ φ }})
-    ∨ (⌜v = VFalse⌝ ∗ EWP eval η e2 @ E <|Ψ|> {{ φ }}) }} -∗
-    EWP eval η (EIfThenElse eb e1 e2) @ E <|Ψ|> {{ φ }}.
+    EWP[ι]eval η eb @ E <|Ψ|> {{ ensures v,
+      (⌜v = VTrue ⌝ ∗ EWP[ι]eval η e1 @ E <|Ψ|> {{ φ }})
+    ∨ (⌜v = VFalse⌝ ∗ EWP[ι]eval η e2 @ E <|Ψ|> {{ φ }}) }} -∗
+    EWP[ι]eval η (EIfThenElse eb e1 e2) @ E <|Ψ|> {{ φ }}.
   Proof.
     iIntros "H".
     iApply (ewp_EIfThenElse_exn' with "H").
@@ -987,8 +916,8 @@ Section ewp_rules_expr.
   (** * EMatch : expr → list branch → expr *)
 
   Lemma ewp_EMatch η e bs Ψ E Φ :
-    EWP deep_handler η e bs @ E <|Ψ|> {{ Φ }} -∗
-    EWP eval η (EMatch e bs) @ E <|Ψ|> {{ Φ }}.
+    EWP[ι]deep_handler η e bs @ E <|Ψ|> {{ Φ }} -∗
+    EWP[ι]eval η (EMatch e bs) @ E <|Ψ|> {{ Φ }}.
   Proof.
     by iIntros "H"; simpl_eval.
   Qed.
@@ -996,11 +925,11 @@ Section ewp_rules_expr.
   (** * ERaise : expr → expr *)
 
   Lemma ewp_ERaise η e φ E Ψ :
-    EWP eval η e @ E <|Ψ|> {{ RET v => φ (O2Throw v) | EXN v => φ (O2Throw v)}} -∗
-    EWP eval η (ERaise e) @ E <|Ψ|> {{ φ }}.
+    EWP[ι] eval η e @ E <|Ψ|> {{ RET v => φ (O2Throw v) | EXN v => φ (O2Throw v)}} -∗
+    EWP[ι] eval η (ERaise e) @ E <|Ψ|> {{ φ }}.
   Proof.
     iIntros "H". simpl_eval.
-    iApply ewp_bind_exn.
+    iApply ewp_bind'.
     iApply (ewp_mono with "H").
     iIntros ([]) "/= H //".
     by iApply ewp_throw.
@@ -1015,18 +944,18 @@ Section ewp_rules_expr.
   Lemma ewp_EAssert_exn η e φ1 φ E Ψ :
     (φ (O2Ret #()))
      ∧
-    (EWP eval η e @ E <|Ψ|> {{ φ1 }} ∗
+    (EWP[ι]eval η e @ E <|Ψ|> {{ φ1 }} ∗
      (∀ v, φ1 (O2Throw v) -∗ φ (O2Throw v)) ∗
      (∀ v, φ1 (O2Ret v) -∗ ⌜v = VTrue⌝ ∗ φ (O2Ret #())))
-    ⊢ EWP eval η (EAssert e) @ E <|Ψ|> {{ φ }}.
+    ⊢ EWP[ι]eval η (EAssert e) @ E <|Ψ|> {{ φ }}.
   Proof.
     iIntros "H /=". simpl_eval.
     iApply ewp_choose.
     iNext. iSplit.
     - iApply ewp_ret. iApply (bi.and_elim_l with "H").
     - iPoseProof (bi.and_elim_r with "H") as "(H & E & P)".
-      iApply ewp_bind_exn.
-      iApply ewp_bind_exn.
+      iApply ewp_bind'.
+      iApply ewp_bind'.
       iApply (ewp_mono with "H").
       iIntros ([v|v]) "H /=".
       * iDestruct ("P" with "H") as "(-> & H)".
@@ -1038,17 +967,17 @@ Section ewp_rules_expr.
 
   Lemma ewp_EAssert_exn_sep η e φ1 φ E Ψ :
     φ (O2Ret #()) ∗
-    (φ (O2Ret #()) -∗ EWP eval η e @ E <|Ψ|> {{ φ1 }}) ∗
+    (φ (O2Ret #()) -∗ EWP[ι] eval η e @ E <|Ψ|> {{ φ1 }}) ∗
     (∀ v, φ1 (O2Throw v) -∗ φ (O2Throw v)) ∗
     (∀ v, φ1 (O2Ret v) -∗ ⌜v = VTrue⌝ ∗ φ (O2Ret #()))
-    ⊢ EWP eval η (EAssert e) @ E <|Ψ|> {{ φ }}.
+    ⊢ EWP[ι] eval η (EAssert e) @ E <|Ψ|> {{ φ }}.
   Proof.
     iIntros "(R & H & He & P) /=". simpl_eval.
     iApply ewp_choose.
     iNext. iSplit. by iApply ewp_ret.
     iSpecialize ("H" with "R").
-    iApply ewp_bind_exn.
-    iApply ewp_bind_exn.
+    iApply ewp_bind'.
+    iApply ewp_bind'.
     iApply (ewp_mono with "H").
     iIntros ([v|v]) "H /=".
     - iDestruct ("P" with "H") as "(-> & H)".
@@ -1058,8 +987,8 @@ Section ewp_rules_expr.
   Qed.
 
   Lemma ewp_EAssert η e R E Ψ :
-    R ∧ EWP eval η e @ E <|Ψ|> {{ ensures v, ⌜v = VTrue⌝ ∗ R }} -∗
-    EWP eval η (EAssert e) @ E <|Ψ|> {{ ensures _, R }}.
+    R ∧ EWP[ι]eval η e @ E <|Ψ|> {{ ensures v, ⌜v = VTrue⌝ ∗ R }} -∗
+    EWP[ι]eval η (EAssert e) @ E <|Ψ|> {{ ensures _, R }}.
   Proof.
     iIntros "H".
     iApply ewp_EAssert_exn.
@@ -1071,8 +1000,8 @@ Section ewp_rules_expr.
   Qed.
 
   Lemma ewp_EAssert_sep η e R E Ψ :
-    R ∗ (R -∗ EWP eval η e @ E <|Ψ|> {{ ensures v, ⌜v = VTrue⌝ ∗ R }}) -∗
-    EWP eval η (EAssert e) @ E <|Ψ|> {{ ensures _, R }}.
+    R ∗ (R -∗ EWP[ι]eval η e @ E <|Ψ|> {{ ensures v, ⌜v = VTrue⌝ ∗ R }}) -∗
+    EWP[ι]eval η (EAssert e) @ E <|Ψ|> {{ ensures _, R }}.
   Proof.
     iIntros "(? & ?)".
     iApply ewp_EAssert_exn_sep. iFrame. eauto.
@@ -1081,13 +1010,13 @@ Section ewp_rules_expr.
   (** * ERef : expr → expr *)
 
   Lemma ewp_ERef_exn η e φ1 φ E Ψ :
-    EWP eval η e @ E <|Ψ|> {{ φ1 }} -∗
+    EWP[ι] eval η e @ E <|Ψ|> {{ φ1 }} -∗
     (∀ v, φ1 (O2Throw v) -∗ φ (O2Throw v)) -∗
     (∀ v, φ1 (O2Ret v) -∗ ∀ l, l ↦ (V v) -∗ φ (O2Ret (VLoc l))) -∗
-    EWP eval η (ERef e) @ E <|Ψ|> {{ φ }}.
+    EWP[ι] eval η (ERef e) @ E <|Ψ|> {{ φ }}.
   Proof.
     iIntros "H E P". simpl_eval.
-    iApply ewp_bind_exn.
+    iApply ewp_bind'.
     iApply (ewp_mono with "H").
     iIntros ([v|v]) "H".
     - iApply ewp_alloc. iNext. iIntros (l) "Hl".
@@ -1099,17 +1028,17 @@ Section ewp_rules_expr.
   Qed.
 
   Lemma ewp_ERef η e φ1 φ E Ψ :
-    EWP eval η e @ E <|Ψ|> {{ ensures v, φ1 v }} -∗
+    EWP[ι] eval η e @ E <|Ψ|> {{ ensures v, φ1 v }} -∗
     (∀ v, φ1 v -∗ ∀ l, l ↦ (V v) -∗ φ (VLoc l)) -∗
-    EWP eval η (ERef e) @ E <|Ψ|> {{ ensures v, φ v }}.
+    EWP[ι] eval η (ERef e) @ E <|Ψ|> {{ ensures v, φ v }}.
   Proof.
     iIntros "H P".
     iApply (ewp_ERef_exn with "H"); auto.
   Qed.
 
   Lemma ewp_ERef' η e φ1 E Ψ :
-    EWP eval η e @ E <|Ψ|> {{ ensures v, φ1 v }} -∗
-      EWP eval η (ERef e) @ E <|Ψ|>
+    EWP[ι]eval η e @ E <|Ψ|> {{ ensures v, φ1 v }} -∗
+      EWP[ι]eval η (ERef e) @ E <|Ψ|>
       {{ ensures r, ∃ l v,
           ⌜r = VLoc l⌝ ∗ l ↦ (V v) ∗ φ1 v }}.
   Proof.
@@ -1123,13 +1052,13 @@ Section ewp_rules_expr.
   (** * ELoad : expr → expr *)
 
   Lemma ewp_ELoad_exn η e φ1 φ E Ψ :
-    EWP as_loc (eval η e) @ E <|Ψ|> {{ φ1 }} -∗
+    EWP[ι] as_loc (eval η e) @ E <|Ψ|> {{ φ1 }} -∗
     (∀ v, φ1 (O2Throw v) -∗ φ (O2Throw v)) -∗
     (∀ l, φ1 (O2Ret l) -∗ ∃ q v, pointsto l q (V v) ∗ ▷(pointsto l q (V v) -∗ φ (O2Ret v))) -∗
-    EWP eval η (ELoad e) @ E <|Ψ|> {{ φ }}.
+    EWP[ι] eval η (ELoad e) @ E <|Ψ|> {{ φ }}.
   Proof.
     iIntros "H E P /=". simpl_eval.
-    iApply ewp_bind_exn.
+    iApply ewp_bind'.
     iApply (ewp_mono with "H").
     iIntros ([l|v]) "H1".
     - iSpecialize ("P" with "H1").
@@ -1141,17 +1070,17 @@ Section ewp_rules_expr.
   Qed.
 
   Lemma ewp_ELoad η e φ1 φ E Ψ :
-    EWP as_loc (eval η e) @ E <|Ψ|> {{ ensures l, φ1 l }} -∗
+    EWP[ι]as_loc (eval η e) @ E <|Ψ|> {{ ensures l, φ1 l }} -∗
     (∀ l, φ1 l -∗ ∃ q v, pointsto l q (V v) ∗ ▷(pointsto l q (V v) -∗ φ v)) -∗
-    EWP eval η (ELoad e) @ E <|Ψ|> {{ ensures v, φ v }}.
+    EWP[ι]eval η (ELoad e) @ E <|Ψ|> {{ ensures v, φ v }}.
   Proof.
     iIntros "H P".
     iApply (ewp_ELoad_exn with "H"); auto.
   Qed.
 
   Lemma ewp_ELoad_simple η e (l : loc) q (v : val) E Ψ :
-    EWP eval η e @ E <|Ψ|> {{ RET= #l }} -∗
-    pointsto l q (V v) -∗ EWP eval η (ELoad e) @ E <|Ψ|> {{ RET= v, pointsto l q (V v) }}.
+    EWP[ι]eval η e @ E <|Ψ|> {{ RET= #l }} -∗
+    pointsto l q (V v) -∗ EWP[ι]eval η (ELoad e) @ E <|Ψ|> {{ RET= v, pointsto l q (V v) }}.
   Proof.
     iIntros "H Hl". iApply (ewp_ELoad _ _ (λ l1, ⌜l = l1⌝%I) with "[H]").
     - iApply ewp_bind. iApply (ewp_mono_ret with "H").
@@ -1161,7 +1090,7 @@ Section ewp_rules_expr.
 
   (** * EStore : expr → expr → expr *)
 
-  Lemma ewpi_EStore_exn ι η e1 e2 φ1 φ2 φ E Ψ :
+  Lemma ewp_EStore_exn η e1 e2 φ1 φ2 φ E Ψ :
     EWP[ι] as_loc (eval η e1) @ E <|Ψ|> {{ φ1 }} -∗
     EWP[ι] eval η e2 @ E <|Ψ|> {{ φ2 }} -∗
     (∀ v, φ1 (O2Throw v) -∗ φ (O2Throw v)) -∗
@@ -1171,9 +1100,9 @@ Section ewp_rules_expr.
     EWP[ι] eval η (EStore e1 e2) @ E <|Ψ|> {{ φ }}.
   Proof.
     iIntros "H1 H2 E1 E2 P /=". simpl_eval.
-    iApply (ewpi_Par with "H1 H2 [E1] [E2]").
-    - iIntros (e) "H1". iApply ewpi_throw. iApply ("E1" with "H1").
-    - iIntros (e) "H2". iApply ewpi_throw. iApply ("E2" with "H2").
+    iApply (ewp_Par with "H1 H2 [E1] [E2]").
+    - iIntros (e) "H1". iApply ewp_throw. iApply ("E1" with "H1").
+    - iIntros (e) "H2". iApply ewp_throw. iApply ("E2" with "H2").
     - iIntros (l1 v2) "H1 H2".
       iSpecialize ("P" $! l1 v2 with "[$]").
       iDestruct "P" as (v1) "(Hl1 & P)".
@@ -1182,24 +1111,7 @@ Section ewp_rules_expr.
       iApply ("P" with "Hl1").
   Qed.
 
-  Lemma ewp_EStore_exn η e1 e2 φ1 φ2 φ E Ψ :
-    EWP as_loc (eval η e1) @ E <|Ψ|> {{ φ1 }} -∗
-    EWP eval η e2 @ E <|Ψ|> {{ φ2 }} -∗
-    (∀ v, φ1 (O2Throw v) -∗ φ (O2Throw v)) -∗
-    (∀ v, φ2 (O2Throw v) -∗ φ (O2Throw v)) -∗
-    (∀ l1 v2, φ1 (O2Ret l1) ∗ φ2 (O2Ret v2) -∗
-      ∃ v1, l1 ↦ (V v1) ∗ ▷(l1 ↦ (V v2) -∗ φ (O2Ret VUnit))) -∗
-    EWP eval η (EStore e1 e2) @ E <|Ψ|> {{ φ }}.
-  Proof.
-    iIntros "H1 H2 E1 E2 P %ι".
-    iApply (ewpi_EStore_exn with "[H1] [H2] [E1] [E2] P").
-    - by iApply ewpi_ewp.
-    - by iApply ewpi_ewp.
-    - iIntros (e) "H1". by iApply "E1".
-    - iIntros (e) "H2". by iApply "E2".
-  Qed.
-
-  Lemma ewpi_EStore {ι η e1 e2} (φ1 : loc -d> iPropO Σ) (φ2 : val -d> iPropO Σ) φ E Ψ :
+  Lemma ewp_EStore {η e1 e2} (φ1 : loc -d> iPropO Σ) (φ2 : val -d> iPropO Σ) φ E Ψ :
     EWP[ι] eval η e1 @ E <|Ψ|> {{ ensures #l1, φ1 l1 }} -∗
     EWP[ι] eval η e2 @ E <|Ψ|> {{ ensures v2, φ2 v2 }} -∗
     (∀ l1 v2, φ1 l1 ∗ φ2 v2 -∗
@@ -1207,11 +1119,11 @@ Section ewp_rules_expr.
     EWP[ι] eval η (EStore e1 e2) @ E <|Ψ|> {{ ensures v, φ v }}.
   Proof.
     iIntros "H1 H2 P".
-    iApply (ewpi_EStore_exn with "[H1] H2").
-    - iApply ewpi_bind; iApply (ewpi_mono with "H1").
+    iApply (ewp_EStore_exn with "[H1] H2").
+    - iApply ewp_bind; iApply (ewp_mono with "H1").
       iIntros ([|]); [ iIntros "H1 /=" | iIntros "[]" ].
       iDestruct "H1" as "(%v & -> & H1)".
-      iApply ewpi_ret.
+      iApply ewp_ret.
       instantiate (1 := (λ o, match o with | O2Ret l => φ1 l | _ => False end)%I).
       iApply "H1".
     - iIntros (? []).
@@ -1219,53 +1131,29 @@ Section ewp_rules_expr.
     - simpl. iExact "P".
   Qed.
 
-  Lemma ewp_EStore {η e1 e2} (φ1 : loc -d> iPropO Σ) (φ2 : val -d> iPropO Σ) φ E Ψ :
-    EWP eval η e1 @ E <|Ψ|> {{ ensures #l1, φ1 l1 }} -∗
-    EWP eval η e2 @ E <|Ψ|> {{ ensures v2, φ2 v2 }} -∗
-    (∀ l1 v2, φ1 l1 ∗ φ2 v2 -∗
-      ∃ v1, l1 ↦ (V v1) ∗ ▷(l1 ↦ (V v2) -∗ φ VUnit)) -∗
-    EWP eval η (EStore e1 e2) @ E <|Ψ|> {{ ensures v, φ v }}.
-  Proof.
-    iIntros "H1 H2 P %ι".
-    iApply (ewpi_EStore with "[H1] [H2] P").
-    by iApply ewpi_ewp.
-    by iApply ewpi_ewp.
-  Qed.
-
   (* Here, [l↦v] is threaded through [e2], as one is more likely to use
      ownership of [l] in [e2] than in [e1] (i.e. we rarely write things like
      [(!r := 1; r) := 2]) *)
-  Lemma ewpi_EStore_simple ι η e1 e2 (l : loc) (v v' : val) E Ψ :
+  Lemma ewp_EStore_simple η e1 e2 (l : loc) (v v' : val) E Ψ :
     EWP[ι] eval η e1 @ E <|Ψ|> {{ RET= #l }} -∗
     EWP[ι] eval η e2 @ E <|Ψ|> {{ RET= v', l ↦ (V v) }} -∗
     EWP[ι] eval η (EStore e1 e2) @ E <|Ψ|> {{ RET= #(), l ↦ (V v') }}.
   Proof.
     iIntros "H1 H2".
-    iApply (ewpi_EStore (λ l1, ⌜l = l1⌝%I)  with "[H1] H2").
-    - iApply (ewpi_mono with "H1").
+    iApply (ewp_EStore (λ l1, ⌜l = l1⌝%I)  with "[H1] H2").
+    - iApply (ewp_mono with "H1").
       iIntros ([|]); [ | iIntros "[]" ].
       iIntros "(-> & _)".
       iExists l; auto.
     - iIntros (? ?) "(-> & -> & Hl)". iExists _. iFrame. auto.
   Qed.
 
-  Lemma ewp_EStore_simple η e1 e2 (l : loc) (v v' : val) E Ψ :
-    EWP eval η e1 @ E <|Ψ|> {{ RET= #l }} -∗
-    EWP eval η e2 @ E <|Ψ|> {{ RET= v', l ↦ (V v) }} -∗
-    EWP eval η (EStore e1 e2) @ E <|Ψ|> {{ RET= #(), l ↦ (V v') }}.
-  Proof.
-    iIntros "H1 H2 %ι".
-    iApply (ewpi_EStore_simple with "[H1] [H2]");
-      by iApply ewpi_ewp.
-  Qed.
-
-
   (** * EPerform : expr -> expr *)
 
   Lemma ewp_EPerform η e E ψ (φ1 : val -d> iPropO Σ) φ :
-    EWP eval η e @ E <|ψ|> {{ ensures v, φ1 v }} -∗
-    (∀ v, φ1 v -∗ EWP perform v @ E <|ψ|> {{ φ }} ) -∗
-    EWP eval η (EPerform e) @ E <|ψ|> {{ φ }}.
+    EWP[ι]eval η e @ E <|ψ|> {{ ensures v, φ1 v }} -∗
+    (∀ v, φ1 v -∗ EWP[ι]perform v @ E <|ψ|> {{ φ }} ) -∗
+    EWP[ι]eval η (EPerform e) @ E <|ψ|> {{ φ }}.
   Proof.
     iIntros "He Hv".
     simpl_eval. iApply ewp_bind.
@@ -1275,33 +1163,12 @@ Section ewp_rules_expr.
 
   (** * EContinue : expr -> expr -> expr *)
 
-  Lemma ewpi_EContinue' ι η e1 e2 E ψ (φ1 : cont -d> iPropO Σ) (φ2 : val -d> iPropO Σ)  φ :
+  Lemma ewp_EContinue' η e1 e2 E ψ (φ1 : cont -d> iPropO Σ) (φ2 : val -d> iPropO Σ)  φ :
     EWP[ι] (eval η e1) @ E <|ψ|> {{ ensures #k, φ1 k }} -∗
     EWP[ι] eval η e2 @ E <|ψ|> {{ ensures v2, φ2 v2 }} -∗
     (∀ (k : cont) v, φ1 k -∗ φ2 v -∗
                 EWP[ι] stop CResume (k, O2Ret v) @ E <|ψ|> {{ φ }}) -∗
     EWP[ι] eval η (EContinue e1 e2) @ E <|ψ|> {{ φ }}.
-  Proof.
-    iIntros "Hk Hv Hmon".
-    simpl_eval.
-    iApply (ewpi_Par with "[Hk] Hv"); try done.
-    { unfold as_cont. iApply ewpi_bind.
-      iApply (ewpi_mono with "Hk").
-      iIntros ([|]); last done.
-      iIntros "(%v & -> & Hφ1)".
-      iApply ewpi_ret. instantiate (1 := (λ o, match o with O2Ret v => φ1 v | O2Throw _ => False end)%I).
-      iApply "Hφ1". }
-    1-2: simpl; iIntros; try done.
-    simpl; iIntros (k v) "Hφ1 Hφ2".
-    iApply ("Hmon" with "Hφ1 Hφ2").
-  Qed.
-
-    Lemma ewp_EContinue' η e1 e2 E ψ (φ1 : cont -d> iPropO Σ) (φ2 : val -d> iPropO Σ)  φ :
-    EWP (eval η e1) @ E <|ψ|> {{ ensures #k, φ1 k }} -∗
-    EWP eval η e2 @ E <|ψ|> {{ ensures v2, φ2 v2 }} -∗
-    (∀ (k : cont) v, φ1 k -∗ φ2 v -∗
-                EWP stop CResume (k, O2Ret v) @ E <|ψ|> {{ φ }}) -∗
-    EWP eval η (EContinue e1 e2) @ E <|ψ|> {{ φ }}.
   Proof.
     iIntros "Hk Hv Hmon".
     simpl_eval.
@@ -1318,13 +1185,13 @@ Section ewp_rules_expr.
   Qed.
 
   Corollary ewp_EContinue η e1 e2 E ψ (φ1 : cont -d> iPropO Σ) (φ2 : val -d> iPropO Σ)  φ :
-    EWP (eval η e1) @ E <|ψ|> {{ ensures #k, φ1 k }} -∗
-    EWP eval η e2 @ E <|ψ|> {{ ensures v2, φ2 v2 }} -∗
+    EWP[ι](eval η e1) @ E <|ψ|> {{ ensures #k, φ1 k }} -∗
+    EWP[ι]eval η e2 @ E <|ψ|> {{ ensures v2, φ2 v2 }} -∗
     (∀ k v, φ1 k -∗ φ2 v -∗
        ∃ sk, isCont k sk ∗
         (isShot k -∗
-            ▷ EWP (sk (O2Ret v)) @ E <|ψ|> {{ φ }})) -∗
-    EWP eval η (EContinue e1 e2) @ E <|ψ|> {{ φ }}.
+            ▷ EWP[ι](sk (O2Ret v)) @ E <|ψ|> {{ φ }})) -∗
+    EWP[ι]eval η (EContinue e1 e2) @ E <|ψ|> {{ φ }}.
   Proof.
     iIntros "H1 H2 H3".
     iApply (ewp_EContinue' with "H1 H2").
@@ -1338,11 +1205,11 @@ Section ewp_rules_expr.
   Qed.
 
   Lemma ewp_EFork_call φ η e1 e2 E Ψ (φ1 φ2 : val -> iProp Σ) :
-    EWP eval η e1 @ E <|Ψ|> {{ ensures v1, φ1 v1 }} -∗
-    EWP eval η e2 @ E <|Ψ|> {{ ensures v2, φ2 v2 }} -∗
-    ▷ (∀ ι v1 v2, valid_thread ι φ -∗ φ1 v1 -∗ φ2 v2 -∗
-                  EWP[ι] call v1 v2 @ E <| ⊥ |> {{ λ o, □ φ o }}) -∗
-    EWP eval η (EFork e1 e2) @ E <|Ψ|> {{ ensures #ι, valid_thread ι φ }}.
+    EWP[ι] eval η e1 @ E <|Ψ|> {{ ensures v1, φ1 v1 }} -∗
+    EWP[ι] eval η e2 @ E <|Ψ|> {{ ensures v2, φ2 v2 }} -∗
+    ▷ (∀ ι' v1 v2, valid_thread ι' φ -∗ φ1 v1 -∗ φ2 v2 -∗
+                  EWP[ι'] call v1 v2 @ E <| ⊥ |> {{ λ o, □ φ o }}) -∗
+    EWP[ι] eval η (EFork e1 e2) @ E <|Ψ|> {{ ensures #ι, valid_thread ι φ }}.
   Proof.
     iIntros "H1 H2 Hcall".
     simpl_eval.
@@ -1351,32 +1218,33 @@ Section ewp_rules_expr.
     { iIntros (e) "[]". }
     iIntros (v1 v2) "H1 H2"; simpl.
     iApply ewp_fork.
-    iIntros "!> !>" (ι) "#Hvalid".
+    iIntros "!> !>" (ι') "#Hvalid".
     iSplitR ""; [ | ].
     iApply ("Hcall" with "Hvalid H1 H2").
     iExists _; iFrame "#"; iPureIntro; reflexivity.
   Qed.
 
   Lemma ewp_EFork `{Encode A} P φ η e1 e2 E Ψ (φ2 : A -> iProp Σ) :
-    EWP eval η e1 @ E <|Ψ|> {{ ensures f, iSpec τ[A] f P }} -∗
-    EWP eval η e2 @ E <|Ψ|> {{ ensures #v2, φ2 v2 }} -∗
-    ▷ (∀ ι v m, valid_thread ι φ -∗ φ2 v -∗ P v m -∗ EWP[ι] m @ E <| ⊥ |> {{ λ o, □ φ o }}) -∗
-    EWP eval η (EFork e1 e2) @ E <|Ψ|> {{ ensures #v, valid_thread v φ }}.
+    EWP[ι] eval η e1 @ E <|Ψ|> {{ ensures f, iSpec τ[A] f P }} -∗
+    EWP[ι] eval η e2 @ E <|Ψ|> {{ ensures #v2, φ2 v2 }} -∗
+    ▷ (∀ ι' v m, valid_thread ι' φ -∗ φ2 v -∗
+                 P v m -∗ EWP[ι'] m @ E <| ⊥ |> {{ λ o, □ φ o }}) -∗
+    EWP[ι] eval η (EFork e1 e2) @ E <|Ψ|> {{ ensures #v, valid_thread v φ }}.
   Proof.
     iIntros "H1 H2 Hcall".
     iApply (ewp_EFork_call with "H1 H2").
-    iIntros "!>" (ι f v2) "#Hvalid HSpec (%v & -> & H2)".
+    iIntros "!>" (ι' f v2) "#Hvalid HSpec (%v & -> & H2)".
     rewrite iSpec_equation_1.
     iSpecialize ("HSpec" $! v).
-    iApply ("Hcall" $! ι v (call f #v) with "Hvalid H2 HSpec").
+    iApply ("Hcall" $! ι' v (call f #v) with "Hvalid H2 HSpec").
   Qed.
 
   Lemma ewp_EFork_call' φ η e1 e2 E Ψ (φ1 φ2 : val -> iProp Σ) :
-    EWP eval η e1 @ E <|Ψ|> {{ ensures v1, φ1 v1 }} -∗
-    EWP eval η e2 @ E <|Ψ|> {{ ensures v2, φ2 v2 }} -∗
-    ▷ (∀ v1 v2, φ1 v1 -∗ φ2 v2 -∗
-                  EWP call v1 v2 @ E <| ⊥ |> {{ λ o, □ φ o }}) -∗
-    EWP eval η (EFork e1 e2) @ E <|Ψ|> {{ ensures #ι, valid_thread ι φ }}.
+    EWP[ι] eval η e1 @ E <|Ψ|> {{ ensures v1, φ1 v1 }} -∗
+    EWP[ι] eval η e2 @ E <|Ψ|> {{ ensures v2, φ2 v2 }} -∗
+    ▷ (∀ ι' v1 v2, φ1 v1 -∗ φ2 v2 -∗
+                  EWP[ι'] call v1 v2 @ E <| ⊥ |> {{ λ o, □ φ o }}) -∗
+    EWP[ι] eval η (EFork e1 e2) @ E <|Ψ|> {{ ensures #ι, valid_thread ι φ }}.
   Proof.
     iIntros "H1 H2 Hcall".
     simpl_eval.
@@ -1385,30 +1253,30 @@ Section ewp_rules_expr.
     { iIntros (e) "[]". }
     iIntros (v1 v2) "H1 H2"; simpl.
     iApply ewp_fork.
-    iIntros "!> !>" (ι) "#Hvalid".
+    iIntros "!> !>" (ι') "#Hvalid".
     iSplitR ""; [ | ].
     iApply ("Hcall" with "H1 H2").
     iExists _; iFrame "#"; iPureIntro; reflexivity.
   Qed.
 
   Lemma ewp_EFork' `{Encode A} P φ η e1 e2 E Ψ (φ2 : A -> iProp Σ) :
-    EWP eval η e1 @ E <|Ψ|> {{ ensures f, iSpec τ[A] f P }} -∗
-    EWP eval η e2 @ E <|Ψ|> {{ ensures #v2, φ2 v2 }} -∗
-    ▷ (∀ v m, φ2 v -∗ P v m -∗ EWP m @ E <| ⊥ |> {{ λ o, □ φ o }}) -∗
-    EWP eval η (EFork e1 e2) @ E <|Ψ|> {{ ensures #v, valid_thread v φ }}.
+    EWP[ι]eval η e1 @ E <|Ψ|> {{ ensures f, iSpec τ[A] f P }} -∗
+    EWP[ι]eval η e2 @ E <|Ψ|> {{ ensures #v2, φ2 v2 }} -∗
+    ▷ (∀ ι' v m, φ2 v -∗ P v m -∗ EWP[ι'] m @ E <| ⊥ |> {{ λ o, □ φ o }}) -∗
+    EWP[ι]eval η (EFork e1 e2) @ E <|Ψ|> {{ ensures #v, valid_thread v φ }}.
   Proof.
     iIntros "H1 H2 Hcall".
     iApply (ewp_EFork_call' with "H1 H2").
-    iIntros "!>" (f v2) "HSpec (%v & -> & H2)".
+    iIntros "!>" (ι' f v2) "HSpec (%v & -> & H2)".
     rewrite iSpec_equation_1.
     iSpecialize ("HSpec" $! v).
-    iApply ("Hcall" $! v (call f #v) with "H2 HSpec").
+    iApply ("Hcall" $! ι' v (call f #v) with "H2 HSpec").
   Qed.
 
   Lemma ewp_EJoin e η E Ψ φ Φ :
-    EWP eval η e @ E <|Ψ|> {{ ensures #ι, valid_thread ι φ }} -∗
+    EWP[ι]eval η e @ E <|Ψ|> {{ ensures #ι, valid_thread ι φ }} -∗
     ▷ (∀ o, □ φ o -∗ Φ o) -∗
-    EWP eval η (EJoin e) @ E <|Ψ|> {{ Φ }}.
+    EWP[ι]eval η (EJoin e) @ E <|Ψ|> {{ Φ }}.
   Proof.
     iIntros "Hid Hjoined".
     simpl_eval.
